meta-theory/pure_demandScript.sml
@@ -1,14 +1,12 @@
 (*
    Formalises the notion of "demand" as used in demand/strictness analysis.
 *)
-
 open HolKernel Parse boolLib bossLib term_tactic;
 open arithmeticTheory listTheory stringTheory alistTheory dep_rewrite
      optionTheory pairTheory ltreeTheory llistTheory bagTheory
      BasicProvers pred_setTheory relationTheory rich_listTheory finite_mapTheory;
 open pure_expTheory pure_valueTheory pure_evalTheory pure_eval_lemmasTheory
-     pure_exp_lemmasTheory pure_miscTheory pure_exp_relTheory pure_congruenceTheory
-     pure_no_err_relTheory;
+     pure_exp_lemmasTheory pure_miscTheory pure_exp_relTheory pure_congruenceTheory;
 
 val _ = new_theory "pure_demand";
 
@@ -17,1288 +15,198 @@ Definition Projs_def:
   Projs ((x,i)::ps) e = Projs ps (Proj x i e)
 End
 
-Theorem demands_proj_end:
-  ∀ ps x i e. Projs (ps++[(x,i)]) e = Proj x i (Projs ps e)
-Proof
-  Induct THEN1 rw [Projs_def]
-  \\ gen_tac \\ rename1 ‘hd::ps’
-  \\ PairCases_on ‘hd’
-  \\ rw [Projs_def]
-QED
-
-Theorem double_Projs:
-  ∀ps' ps e. Projs (ps' ++ ps) e = Projs ps (Projs ps' e)
-Proof
-  Induct >- rw [Projs_def]
-  \\ gen_tac \\ rename1 ‘hd::ps'’
-  \\ PairCases_on ‘hd’
-  \\ rw [Projs_def]
-QED
-
-Theorem no_err_eq_Projs_cong:
-  ∀ps x y. x no_err_rel y ⇒ Projs ps x no_err_rel Projs ps y
-Proof
-  Induct \\ fs [Projs_def,FORALL_PROD]
-  \\ rw [] \\ first_x_assum irule
-  \\ irule no_err_eq_Prim_cong \\ fs [no_err_eq_refl,Let_Var]
-QED
-
-Theorem no_err_Projs_Seq:
-  ∀ps e e'. Projs ps (Seq e e') no_err_rel Seq e (Projs ps e')
-Proof
-  Induct
-  THEN1 (rw [Projs_def] \\ fs [no_err_eq_refl])
-  \\ rpt gen_tac
-  \\ rename1 ‘hd::ps’
-  \\ PairCases_on ‘hd’
-  \\ rw [Projs_def]
-  \\ irule no_err_eq_trans \\ qexists_tac ‘Projs ps (Seq e (Proj hd0 hd1 e'))’
-  \\ fs [no_err_Proj_Seq2, no_err_eq_sym, no_err_eq_Projs_cong, no_err_Seq_id]
-QED
-
-Theorem no_err_Let_Projs:
-  ∀ps x w y. Let w y (Projs ps x) no_err_rel Projs ps (Let w y x)
-Proof
-  Induct \\ fs [Projs_def,no_err_eq_refl,FORALL_PROD] \\ rw []
-  \\ irule no_err_eq_trans
-  \\ qexists_tac ‘Projs ps (Let w y (Proj p_1 p_2 x))’
-  \\ conj_tac THEN1 fs []
-  \\ irule no_err_eq_Projs_cong
-  \\ fs [no_err_Let_Prim_alt]
-QED
-
-Theorem Projs_subst:
-  ∀ps f e. subst f (Projs ps e) = Projs ps (subst f e)
-Proof
-  Induct THEN1 rw [Projs_def]
-  \\ gen_tac
-  \\ rename1 ‘Projs (hd::_) _’
-  \\ PairCases_on ‘hd’
-  \\ rw [Projs_def, subst_def]
-QED
-
 val _ = set_fixity "demands" (Infixl 480);
 
 Definition demands_def:
-  (e demands (p,v)) = (e no_err_rel Seq (Projs p (Var v)) e)
+  (e demands (p,v)) = (e ≅ Seq (Projs p (Var v)) e)
 End
-
-val _ = set_fixity "needs" (Infixl 480);
-Definition needs_def:
-  (e needs (ps, e')) = (e no_err_rel Seq (Projs ps e') e)
-End
-
-Theorem needs_Var_is_demands:
-  e needs (ps, Var v) ⇔ e demands (ps, v)
-Proof
-  rw [needs_def, demands_def] \\ fs []
-QED
-
-Theorem needs_refl:
-  ∀e. e needs ([],e)
-Proof
-  rw [needs_def, Projs_def]
-  \\ metis_tac [no_err_Seq_id, no_err_eq_sym]
-QED
-
-Theorem needs_Var:
-  (Var v) needs ([], Var v)
-Proof
-  fs [needs_refl]
-QED
-
-Theorem needs_Proj:
-  e needs d ⇒ (Proj n i e) needs d
-Proof
-  PairCases_on ‘d’
-  \\ rename1 ‘(ps, e')’
-  \\ rw [needs_def, Projs_def]
-  \\ irule no_err_eq_trans
-  \\ qexists_tac ‘Seq e (Proj n i e)’
-  \\ conj_tac >- fs [no_err_Proj_Seq]
-  \\ qabbrev_tac ‘p = Projs ps e'’
-  \\ irule no_err_eq_trans
-  \\ qexists_tac ‘Seq (Seq p e) (Proj n i e)’
-  \\ conj_tac
-  >- (irule no_err_eq_Prim_cong \\ fs [no_err_eq_refl])
-  \\ irule no_err_eq_trans
-  \\ qexists_tac ‘Seq p (Seq e (Proj n i e))’
-  \\ conj_tac >- fs [no_err_Seq_assoc]
-  \\ irule no_err_eq_Prim_cong \\ fs [no_err_eq_refl, no_err_Let_Var]
-  \\ metis_tac [no_err_Proj_Seq, no_err_eq_sym]
-QED
-
-Theorem needs_Projs:
-  ∀ps e d. e needs d ⇒ (Projs ps e) needs d
-Proof
-  Induct
-  >- rw [Projs_def]
-  \\ gen_tac \\ rename1 ‘(hd::ps)’ \\ PairCases_on ‘hd’
-  \\ rw [Projs_def]
-  \\ first_assum $ irule_at Any
-  \\ irule needs_Proj
-  \\ fs []
-QED
-
-Theorem needs_trans:
-  e needs (ps,e') ∧ e' needs (ps',e'') ⇒ e needs (ps',e'')
-Proof
-  rw [needs_def]
-  \\ irule no_err_eq_trans
-  \\ first_assum $ irule_at Any
-  \\ irule no_err_eq_trans
-  \\ qexists_tac ‘Seq (Seq (Projs ps' e'') (Projs ps e')) e’
-  \\ conj_tac >-
-   (irule no_err_eq_Prim_cong \\ fs [no_err_eq_refl]
-    \\ assume_tac needs_Projs \\ metis_tac [needs_def])
-  \\ irule no_err_eq_trans
-  \\ qexists_tac ‘Seq (Projs ps' e'') (Seq (Projs ps e') e)’
-  \\ conj_tac >- fs [no_err_Seq_assoc]
-  \\ irule no_err_eq_Prim_cong
-  \\ fs [no_err_eq_refl, no_err_eq_sym]
-QED
-
-Theorem needs_Projs_Var:
-  (Proj s i (Var v)) needs ([(s,i)], Var v)
-Proof
-  rw [needs_def, Projs_def]
-  \\ metis_tac [no_err_Seq_id, no_err_eq_sym]
-QED
-
-Theorem needs_Seq:
-  e needs d ⇒ (Seq e e') needs d
-Proof
-  PairCases_on ‘d’
-  \\ rw [needs_def]
-  \\ irule no_err_eq_trans
-  \\ qexists_tac ‘Seq (Seq (Projs d0 d1) e) e'’
-  \\ conj_tac >-
-   (irule no_err_eq_Prim_cong \\ fs [no_err_eq_refl])
-  \\ fs [no_err_Seq_assoc]
-QED
-
-Theorem needs_Let1:
-  e needs d ∧ e' demands ([],w) ⇒ (Let w e e') needs d
-Proof
-  PairCases_on ‘d’
-  \\ rw [demands_def,needs_def,Projs_def]
-  \\ irule no_err_eq_trans
-  \\ qabbrev_tac ‘p = (Projs d0 d1)’
-  \\ qexists_tac ‘Let w e (Seq (Var w) e')’
-  \\ conj_tac THEN1
-   (irule no_err_eq_App_cong \\ fs [no_err_eq_refl]
-    \\ irule no_err_eq_Lam_cong \\ fs [no_err_eq_refl])
-  \\ irule no_err_eq_trans
-  \\ qexists_tac ‘Seq (Let w e (Var w)) (Let w e e')’
-  \\ conj_tac THEN1 fs [no_err_Let_Seq]
-  \\ irule no_err_eq_trans
-  \\ qexists_tac ‘Seq e (Let w e e')’
-  \\ conj_tac
-  THEN1 (irule no_err_eq_Prim_cong \\ fs [no_err_eq_refl,no_err_Let_Var])
-  \\ irule no_err_eq_trans
-  \\ qexists_tac ‘Seq (Seq p e) (Let w e e')’
-  \\ conj_tac THEN1
-   (irule no_err_eq_Prim_cong \\ fs [no_err_eq_refl])
-  \\ irule no_err_eq_trans
-  \\ qexists_tac ‘Seq p (Seq e (Let w e e'))’
-  \\ conj_tac THEN1 fs [no_err_Seq_assoc]
-  \\ irule no_err_eq_Prim_cong \\ fs [no_err_eq_refl]
-  \\ once_rewrite_tac [no_err_eq_sym]
-  \\ irule no_err_eq_trans
-  \\ irule_at Any no_err_eq_App_cong
-  \\ irule_at Any no_err_eq_Lam_cong
-  \\ irule_at (Pos $ el 2) no_err_eq_refl
-  \\ qexists_tac ‘Seq (Var w) e'’
-  \\ fs [no_err_eq_sym]
-  \\ irule no_err_eq_trans
-  \\ qexists_tac ‘Seq (Let w e (Var w)) (Let w e e')’
-  \\ irule_at (Pos $ el 1) no_err_eq_Prim_cong
-  \\ fs [no_err_eq_refl, no_err_Let_Var, no_err_eq_sym, no_err_Let_Seq]
-QED
-
-Theorem needs_Let_Cons: (* expects program to be in ANF *)
-  e demands ((s,LENGTH xs)::ps,w) ⇒
-  (Let w (Cons s (xs ++ e'::ys)) e) needs (ps,e')
-Proof
-  rw [demands_def,needs_def,Projs_def]
-  \\ qabbrev_tac ‘cons = (Cons s (xs ++ e'::ys))’
-  \\ irule no_err_eq_trans
-  \\ qexists_tac ‘Let w cons (Seq (Projs ps (Proj s (LENGTH xs) (Var w))) e)’
-  \\ conj_tac THEN1
-   (irule no_err_eq_App_cong \\ fs [no_err_eq_refl]
-    \\ irule no_err_eq_Lam_cong \\ fs [no_err_eq_refl])
-  \\ irule no_err_eq_trans
-  \\ irule_at Any no_err_Let_Seq
-  \\ irule no_err_eq_Prim_cong \\ fs [no_err_eq_refl,no_err_Let_Var]
-  \\ fs [GSYM Projs_def]
-  \\ irule no_err_eq_trans
-  \\ irule_at Any no_err_Let_Projs
-  \\ fs [Projs_def]
-  \\ irule no_err_eq_Projs_cong \\ fs [no_err_eq_refl,no_err_Let_Var]
-  \\ irule no_err_eq_trans
-  \\ irule_at Any no_err_eq_Prim_cong \\ fs [PULL_EXISTS]
-  \\ irule_at Any no_err_Let_Var
-  \\ unabbrev_all_tac
-  \\ fs [no_err_Proj_Cons]
-QED
-
-Theorem needs_Let_Proj: (* expects program to be in ANF *)
-  e demands (ps,w) ⇒
-  (Let w (Proj s i e') e) needs ((s,i)::ps,e')
-Proof
-  rw [demands_def,needs_def,Projs_def]
-  \\ irule no_err_eq_trans
-  \\ qexists_tac ‘Let w (Proj s i e') (Seq (Projs ps (Var w)) e)’
-  \\ conj_tac THEN1
-   (irule no_err_eq_App_cong \\ fs [no_err_eq_refl]
-    \\ irule no_err_eq_Lam_cong \\ fs [no_err_eq_refl])
-  \\ irule no_err_eq_trans
-  \\ qexists_tac ‘Seq (Let w (Proj s i e') (Projs ps (Var w)))
-                      (Let w (Proj s i e') e)’
-  \\ conj_tac THEN1 fs [no_err_Let_Seq]
-  \\ irule no_err_eq_Prim_cong \\ fs [no_err_eq_refl,no_err_Let_Var]
-  \\ irule no_err_eq_trans
-  \\ qexists_tac ‘Projs ps (Let w (Proj s i e') (Var w))’
-  \\ conj_tac THEN1 fs [no_err_Let_Projs]
-  \\ irule no_err_eq_Projs_cong
-  \\ fs [no_err_Let_Var]
-QED
-
-Theorem needs_App:
-  f needs d ⇒ (App f e) needs d
-Proof
-  PairCases_on ‘d’ \\ rename1 ‘(ps,e')’
-  \\ rw [needs_def]
-  \\ qabbrev_tac ‘proj = Projs ps e'’
-  \\ irule no_err_eq_trans
-  \\ qexists_tac ‘App (Seq proj f) e’
-  \\ conj_tac THEN1
-   (irule no_err_eq_App_cong \\ rw [no_err_eq_refl])
-  \\ fs [no_err_Seq_App]
-QED
-
-Theorem needs_If:
-  e needs d ⇒ (If e e' e'') needs d
-Proof
-  PairCases_on ‘d’
-  \\ rw [needs_def]
-  \\ qabbrev_tac ‘p = Projs d0 d1’
-  \\ irule no_err_eq_trans
-  \\ irule_at Any no_err_If_Seq
-  \\ irule no_err_eq_Prim_cong
-  \\ fs [no_err_eq_refl, no_err_eq_sym]
-QED
-
-
-
-        (********************************************)
 
 Theorem demands_Var:
   (Var v) demands ([],v)
 Proof
-  metis_tac [needs_Var_is_demands, needs_Var]
+  fs [demands_def,Projs_def]
+  \\ metis_tac [Seq_id,exp_eq_sym]
 QED
 
 Theorem demands_Proj:
-  e demands d ⇒
-  (Proj n i e) demands d
+  e demands (ps,v) ⇒
+  (Proj n i e) demands (ps,v)
 Proof
-  PairCases_on ‘d’
-  \\ metis_tac [needs_Var_is_demands, needs_Proj]
-QED
-
-Theorem demands_Projs:
-  e demands d ⇒
-  (Projs ps2 e) demands d
-Proof
-  PairCases_on ‘d’
-  \\ metis_tac [needs_Var_is_demands, needs_Projs]
+  rw [demands_def,Projs_def]
+  \\ irule exp_eq_trans
+  \\ qexists_tac ‘Seq e (Proj n i e)’
+  \\ conj_tac THEN1 fs [Proj_Seq]
+  \\ qabbrev_tac ‘p = Projs ps (Var v)’
+  \\ irule exp_eq_trans
+  \\ qexists_tac ‘Seq (Seq p e) (Proj n i e)’
+  \\ conj_tac THEN1
+   (irule exp_eq_Prim_cong \\ fs [exp_eq_refl])
+  \\ irule exp_eq_trans
+  \\ qexists_tac ‘Seq p (Seq e (Proj n i e))’
+  \\ conj_tac THEN1 fs [Seq_assoc]
+  \\ irule exp_eq_Prim_cong \\ fs [exp_eq_refl,Let_Var]
+  \\ metis_tac [Proj_Seq,exp_eq_sym]
 QED
 
 Theorem demands_Proj_Var:
   (Proj s i (Var v)) demands ([(s,i)],v)
 Proof
   rw [demands_def,Projs_def]
-  \\ metis_tac [no_err_Seq_id,no_err_eq_sym]
+  \\ metis_tac [Seq_id,exp_eq_sym]
 QED
 
-Theorem demands_Seq:
-  e demands d ⇒ (Seq e e') demands d
+Theorem exp_eq_Projs_cong:
+  ∀ps x y. x ≅ y ⇒ Projs ps x ≅ Projs ps y
 Proof
-  PairCases_on ‘d’
-  \\ metis_tac [needs_Var_is_demands, needs_Seq]
+  Induct \\ fs [Projs_def,FORALL_PROD]
+  \\ rw [] \\ first_x_assum irule
+  \\ irule exp_eq_Prim_cong \\ fs [exp_eq_refl,Let_Var]
+QED
+
+Theorem Let_Projs:
+  ∀ps x w y. Let w y (Projs ps x) ≅ Projs ps (Let w y x)
+Proof
+  Induct \\ fs [Projs_def,exp_eq_refl,FORALL_PROD] \\ rw []
+  \\ irule exp_eq_trans
+  \\ qexists_tac ‘Projs ps (Let w y (Proj p_1 p_2 x))’
+  \\ conj_tac THEN1 fs []
+  \\ irule exp_eq_Projs_cong
+  \\ fs [Let_Prim_alt]
 QED
 
 Theorem demands_Let1:
   e demands d ∧ e' demands ([],w) ⇒ (Let w e e') demands d
 Proof
   PairCases_on ‘d’
-  \\ metis_tac [needs_def, needs_Var_is_demands, needs_Let1]
+  \\ rw [demands_def,Projs_def]
+  \\ irule exp_eq_trans
+  \\ qabbrev_tac ‘p = (Projs d0 (Var d1))’
+  \\ qexists_tac ‘Let w e (Seq (Var w) e')’
+  \\ conj_tac THEN1
+   (irule exp_eq_App_cong \\ fs [exp_eq_refl]
+    \\ irule exp_eq_Lam_cong \\ fs [exp_eq_refl])
+  \\ irule exp_eq_trans
+  \\ qexists_tac ‘Seq (Let w e (Var w)) (Let w e e')’
+  \\ conj_tac THEN1 fs [Let_Seq]
+  \\ irule exp_eq_trans
+  \\ qexists_tac ‘Seq e (Let w e e')’
+  \\ conj_tac
+  THEN1 (irule exp_eq_Prim_cong \\ fs [exp_eq_refl,Let_Var])
+  \\ irule exp_eq_trans
+  \\ qexists_tac ‘Seq (Seq p e) (Let w e e')’
+  \\ conj_tac THEN1
+   (irule exp_eq_Prim_cong \\ fs [exp_eq_refl])
+  \\ irule exp_eq_trans
+  \\ qexists_tac ‘Seq p (Seq e (Let w e e'))’
+  \\ conj_tac THEN1 fs [Seq_assoc]
+  \\ irule exp_eq_Prim_cong \\ fs [exp_eq_refl]
+  \\ once_rewrite_tac [exp_eq_sym]
+  \\ irule exp_eq_trans
+  \\ qexists_tac ‘Let w e (Seq (Var w) e')’
+  \\ conj_tac THEN1
+   (irule exp_eq_App_cong \\ fs [exp_eq_refl]
+    \\ irule exp_eq_Lam_cong \\ fs [exp_eq_refl])
+  \\ irule exp_eq_trans
+  \\ qexists_tac ‘Seq (Let w e (Var w)) (Let w e e')’
+  \\ conj_tac THEN1 fs [Let_Seq]
+  \\ irule exp_eq_trans
+  \\ qexists_tac ‘Seq e (Let w e e')’
+  \\ conj_tac THEN1
+    (irule exp_eq_Prim_cong \\ fs [exp_eq_refl,Let_Var])
+  \\ fs [exp_eq_refl]
 QED
 
 Theorem demands_Let2:
   e' demands (p,v) ∧ v ≠ w ⇒ (Let w e e') demands (p,v)
 Proof
   rw [demands_def,Projs_def]
-  \\ irule no_err_eq_trans
+  \\ irule exp_eq_trans
   \\ qexists_tac ‘Let w e (Seq (Projs p (Var v)) e')’
   \\ conj_tac THEN1
-   (irule no_err_eq_App_cong \\ fs [no_err_eq_refl]
-    \\ irule no_err_eq_Lam_cong \\ fs [no_err_eq_refl])
-  \\ irule no_err_eq_trans
+   (irule exp_eq_App_cong \\ fs [exp_eq_refl]
+    \\ irule exp_eq_Lam_cong \\ fs [exp_eq_refl])
+  \\ irule exp_eq_trans
   \\ qexists_tac ‘Seq (Let w e (Projs p (Var v))) (Let w e e')’
-  \\ conj_tac THEN1 fs [no_err_Let_Seq]
-  \\ irule no_err_eq_Prim_cong \\ fs [no_err_eq_refl,no_err_Let_Var]
+  \\ conj_tac THEN1 fs [Let_Seq]
+  \\ irule exp_eq_Prim_cong \\ fs [exp_eq_refl,Let_Var]
   \\ qid_spec_tac ‘p’ \\ Induct
-  THEN1 fs [Projs_def,no_err_Let_Var2]
+  THEN1 fs [Projs_def,Let_Var2]
   \\ fs [FORALL_PROD,Projs_def] \\ rw []
   \\ fs [GSYM Projs_def]
-  \\ irule no_err_eq_trans
+  \\ irule exp_eq_trans
   \\ qexists_tac ‘Projs ((p_1,p_2)::p') (Let w e (Var v))’
-  \\ conj_tac THEN1 fs [no_err_Let_Projs]
-  \\ irule no_err_eq_Projs_cong
-  \\ fs [no_err_Let_Var2]
+  \\ conj_tac THEN1 fs [Let_Projs]
+  \\ irule exp_eq_Projs_cong
+  \\ fs [Let_Var2]
 QED
 
 Theorem demands_Let_Proj: (* expects program to be in ANF *)
   e demands (ps,w) ⇒
   (Let w (Proj s i (Var v)) e) demands ((s,i)::ps,v)
 Proof
-  metis_tac [needs_Let_Proj, needs_Var_is_demands]
+  rw [demands_def,Projs_def]
+  \\ irule exp_eq_trans
+  \\ qexists_tac ‘Let w (Proj s i (Var v)) (Seq (Projs ps (Var w)) e)’
+  \\ conj_tac THEN1
+   (irule exp_eq_App_cong \\ fs [exp_eq_refl]
+    \\ irule exp_eq_Lam_cong \\ fs [exp_eq_refl])
+  \\ irule exp_eq_trans
+  \\ qexists_tac ‘Seq (Let w (Proj s i (Var v)) (Projs ps (Var w)))
+                      (Let w (Proj s i (Var v)) e)’
+  \\ conj_tac THEN1 fs [Let_Seq]
+  \\ irule exp_eq_Prim_cong \\ fs [exp_eq_refl,Let_Var]
+  \\ irule exp_eq_trans
+  \\ qexists_tac ‘Projs ps (Let w (Proj s i (Var v)) (Var w))’
+  \\ conj_tac THEN1 fs [Let_Projs]
+  \\ irule exp_eq_Projs_cong
+  \\ fs [Let_Var]
 QED
 
 Theorem demands_Let_Cons: (* expects program to be in ANF *)
   e demands ((s,LENGTH xs)::ps,w) ⇒
   (Let w (Cons s (xs ++ (Var v)::ys)) e) demands (ps,v)
 Proof
-  metis_tac [needs_Let_Cons, needs_Var_is_demands]
+  rw [demands_def,Projs_def]
+  \\ qabbrev_tac ‘cons = (Cons s (xs ++ Var v::ys))’
+  \\ irule exp_eq_trans
+  \\ qexists_tac ‘Let w cons (Seq (Projs ps (Proj s (LENGTH xs) (Var w))) e)’
+  \\ conj_tac THEN1
+   (irule exp_eq_App_cong \\ fs [exp_eq_refl]
+    \\ irule exp_eq_Lam_cong \\ fs [exp_eq_refl])
+  \\ irule exp_eq_trans
+  \\ irule_at Any Let_Seq
+  \\ irule exp_eq_Prim_cong \\ fs [exp_eq_refl,Let_Var]
+  \\ fs [GSYM Projs_def]
+  \\ irule exp_eq_trans
+  \\ irule_at Any Let_Projs
+  \\ fs [Projs_def]
+  \\ irule exp_eq_Projs_cong \\ fs [exp_eq_refl,Let_Var]
+  \\ irule exp_eq_trans
+  \\ irule_at Any exp_eq_Prim_cong \\ fs [PULL_EXISTS]
+  \\ irule_at Any Let_Var
+  \\ unabbrev_all_tac
+  \\ fs [Proj_Cons]
 QED
-
-Theorem demands_App:
-  f demands d ⇒ (App f e) demands d
-Proof
-  PairCases_on ‘d’
-  \\ metis_tac [needs_App, needs_Var_is_demands]
-QED
-
-Theorem demands_If:
-  e demands d ⇒ (If e e' e'') demands d
-Proof
-  PairCases_on ‘d’
-  \\ metis_tac [needs_If, needs_Var_is_demands]
-QED
-
-Definition well_formed_def:
-  well_formed (Cons s) l = (s ≠ s) ∧
-  well_formed (Proj s i) l = (∃ e. l = [e]) ∧
-  well_formed (IsEq s i) l = (∃e. l = [e]) ∧
-  well_formed If (l: exp list) = (∃e e' e''. l = e::e'::e''::[]) ∧
-  well_formed Seq l = (∃e e'. l = e::e'::[]) ∧
-  well_formed (AtomOp op) l = (op ≠ op)
-End
-
-Theorem demands_Prim:
-  e demands d ∧ well_formed ope (e::l) ⇒ Prim ope (e::l) demands d
-Proof
-  PairCases_on ‘d’
-  \\ rw [demands_def]
-  \\ qabbrev_tac ‘p = Projs d0 (Var d1)’
-  \\ irule no_err_eq_trans \\ qexists_tac ‘Prim ope ((Seq p e)::l)’
-  \\ conj_tac
-  >- (irule no_err_eq_Prim_cong \\ fs [no_err_eq_l_refl])
-  \\ Cases_on ‘ope’ \\ fs [well_formed_def]
-  \\ fs [no_err_If_Seq, no_err_IsEq_Seq, no_err_Proj_Seq2, no_err_Seq_assoc]
-QED
-
-Theorem demands_IsEq:
-  e demands d ⇒ (IsEq n i e) demands d
-Proof
-  strip_tac
-  \\ irule demands_Prim
-  \\ fs [well_formed_def]
-QED
-
-(*
-Definition is_good_def:
-  is_good e = (eval_wh e ≠ wh_Error ∧ eval_wh e ≠ wh_Diverge ∧ closed e)
-End
-
-
-Definition can_commute_def:
-  can_commute  e e' = ∀f.
-                           ¬ (eval_wh (subst f e) = wh_Diverge ∧ eval_wh (subst f e') = wh_Error) ∧
-                           ¬ (eval_wh (subst f e) = wh_Error ∧ eval_wh (subst f e') = wh_Diverge)
-End
-
-Theorem can_commute_sym:
-  can_commute e e' ⇒ can_commute e' e
-Proof
-  metis_tac [can_commute_def]
-QED
-
-Theorem can_commute_Seq_com:
-  ∀e e'. can_commute e e' ⇒ ∀e''. Seq (Seq e e') e'' no_err_rel Seq (Seq e' e) e''
-Proof
-  rw [can_commute_def]
-  \\ irule eval_wh_IMP_no_err_eq
-  \\ gen_tac
-  \\ ‘eval_wh (subst f e) = wh_Diverge ∨ eval_wh (subst f e) = wh_Error ∨ (eval_wh (subst f e) ≠ wh_Diverge ∧ eval_wh (subst f e) ≠ wh_Error)’ by rw [DISJ_EQ_IMP]
-  \\ ‘eval_wh (subst f e') = wh_Diverge ∨ eval_wh (subst f e') = wh_Error ∨ (eval_wh (subst f e') ≠ wh_Diverge ∧ eval_wh (subst f e') ≠ wh_Error)’ by rw [DISJ_EQ_IMP]
-  \\ rw [subst_def, eval_wh_Seq]
-  \\ fs []
-  \\ metis_tac []
-QED
-
-Theorem is_good_means_can_commute:
-  ∀e e'. is_good e ⇒ can_commute e e'
-Proof
-  fs [is_good_def, can_commute_def]
-QED
-
-Theorem demands_Seq_com:
-  ∀e e'. is_good e ∨ is_good e' ⇒ ∀e''. Seq (Seq e e') e'' ∼ Seq (Seq e' e) e''
-Proof
-  rw [is_good_means_can_commute]
-  \\ irule can_commute_Seq_com
-  \\ fs [is_good_means_can_commute, can_commute_sym]
-QED
-
-Theorem needs_Seq2:
-  (can_commute e (Projs ps e'')) ∧ e' needs (ps, e'')
-  ⇒ (Seq e e') needs (ps, e'')
-Proof
-  rw [DISJ_EQ_IMP]
-  \\ fs [needs_def, Projs_def]
-  \\ qabbrev_tac ‘p = Projs ps e''’
-  \\ irule no_err_eq_trans \\ qexists_tac ‘Seq e (Seq p e')’
-  \\ conj_tac
-  >- (irule no_err_eq_Prim_cong \\ fs [no_err_eq_refl])
-  \\ irule no_err_eq_trans \\ qexists_tac ‘Seq (Seq e p) e'’
-  \\ conj_tac
-  >- (‘Seq (Seq e p) e' ∼ Seq e (Seq p e')’ by fs [Seq_assoc]
-      \\ fs [no_err_eq_sym])
-  \\ irule no_err_eq_trans \\ qexists_tac ‘Seq (Seq p e) e'’
-  \\ fs [Seq_assoc]
-  \\ irule can_commute_Seq_com
-  \\ fs [DISJ_EQ_IMP]
-QED
-
-Theorem demands_Seq2:
-  is_good e ∧ e' demands (ps, v)
-   ⇒ (Seq e e') demands (ps, v)
-Proof
-  metis_tac [is_good_means_can_commute,needs_Var_is_demands, needs_Seq2]
-QED
-
-Theorem needs_If2_no_Diverge:
-  (∀f. eval_wh (subst f ce) ≠ wh_Diverge ∧ eval_wh (subst f e) ≠ wh_Diverge)
-  ∧ te ∼ Seq e te' ∧ ee ∼ Seq e ee'
-  ⇒ If ce te ee ∼ Seq e (If ce te' ee')
-Proof
-  rw []
-  \\ irule no_err_eq_trans
-  \\ qexists_tac ‘If ce (Seq e te') (Seq e ee')’
-  \\ conj_tac
-  >- (irule no_err_eq_Prim_cong \\ fs [no_err_eq_refl])
-  \\ irule eval_wh_IMP_no_err_eq
-  \\ rw [subst_def, eval_wh_Seq, eval_wh_If]
-  \\ fs []
-QED
-
-Theorem needs_If2:
-  ((is_good ce ∧ (eval_wh ce = wh_True ∨ eval_wh ce = wh_False)) ∨ is_good e') ∧ te needs ([], e') ∧ ee needs ([], e') ⇒ (If ce te ee) needs ([], e')
-Proof
-  rw [is_good_def, needs_def, Projs_def]
-  \\ irule no_err_eq_trans
-  \\ qexists_tac ‘If ce (Seq e' te) (Seq e' ee)’
-  \\ conj_tac
-  \\ TRY (irule no_err_eq_Prim_cong \\ fs [no_err_eq_refl])
-  \\ irule eval_wh_IMP_no_err_eq
-  \\ rw [subst_def, eval_wh_Seq, eval_wh_If]
-  \\ fs []
-QED
-*)
-
-Theorem needs_projs_reduce:
-  ∀ps ps' e e'. e needs (ps ++ ps', e') ⇒ e needs (ps, e')
-Proof
-  rw [needs_def, double_Projs]
-  \\ qabbrev_tac ‘p = Projs ps e'’
-  \\ irule no_err_eq_trans \\ qexists_tac ‘Seq (Seq p (Projs ps' p)) e’
-  \\ conj_tac
-  >- (irule no_err_eq_trans \\ first_assum $ irule_at Any
-      \\ irule no_err_eq_Prim_cong
-      \\ fs [no_err_eq_refl]
-      \\ ‘p needs ([], p)’ by fs [needs_refl]
-      \\ drule needs_Projs
-      \\ rw [needs_def, Projs_def])
-  \\ irule no_err_eq_trans \\ qexists_tac ‘Seq p (Seq (Projs ps' p) e)’
-  \\ fs [no_err_Seq_assoc]
-  \\ irule no_err_eq_Prim_cong
-  \\ fs [no_err_eq_refl, no_err_eq_sym]
-QED
-
-
-Theorem demands_Projs_empty:
-  ∀ps v. (Projs ps (Var v)) demands ([], v)
-Proof
-  rpt gen_tac
-  \\ ‘(Projs ps (Var v)) demands (ps, v)’ by fs [demands_def, no_err_Seq_id, no_err_eq_sym]
-  \\ irule $ iffLR needs_Var_is_demands
-  \\ irule needs_projs_reduce
-  \\ fs []
-  \\ rw [needs_Var_is_demands]
-  \\ first_assum $ irule_at Any
-QED
-
-Theorem demands_empty_proj:
-  e demands (ps, v) ⇒ e demands ([], v)
-Proof
-  ‘ps = [] ++ ps’ by rw []
-  \\ rw []
-  \\ metis_tac [needs_projs_reduce, needs_Var_is_demands]
-QED
-
-Theorem demands_projs_reduce:
-  e demands (ps ++ ps', v) ⇒ e demands (ps, v)
-Proof
-  metis_tac [needs_projs_reduce, needs_Var_is_demands]
-QED
-
-(*
-Definition fun_demands2_def:
-  f fun_demands (ps,(k:num),(n:num)) ⇒ ∀l hd v. LENGTH l = n ∧ LENGTH hd = k ∧ (l = hd++v::tl) ⇒ Apps f (MAP Var l) demands ([],v)
-End
-*)
-Definition fun_demands_pre_def:
-  fun_demands_pre (k:num) f ps = if k = 0
-                        then ∀n. n ∉ freevars f ⇒ (App f (Var n)) demands (ps, n)
-                        else ∀e. fun_demands_pre (k - 1) (App f e) ps
-End
-
-val _ = set_fixity "fun_demands" (Infixl 478);
-
-Definition fun_demands_def:
-  f fun_demands (ps, k) = fun_demands_pre k f ps
-End
-(*
-Theorem Let_Var_eq:
-  ∀e v. Let v (Var v) e ∼ e
-Proof
-  Induct \\ rw []
-  THEN1 (qsuff_tac ‘v = s ∨ v ≠ s’
-         THEN1 (DISCH_TAC \\ pop_assum DISJ_CASES_TAC
-                THEN1 (rw [] \\ fs [Let_Var])
-                \\ fs [Let_Var2])
-         \\ rw [])
-  THEN1 (irule no_err_eq_trans \\ qexists_tac ‘Prim o' (MAP (Let v (Var v)) l)’
-         \\ conj_tac
-         THEN1 fs [Let_Prim]
-QED
-*)
-(*
-Theorem fun_demands_Lam:
-  e demands (ps, v) ⇒ (Lam v e) fun_demands (ps, 0)
-Proof
-  rw [fun_demands_def, fun_demands_pre_def, demands_def]
-  \\ irule no_err_eq_trans
-  THEN1 (qexists_tac ‘Let v (Var n) (Seq (Projs ps (Var v)) e)’
-         \\ conj_tac
-         THEN1 (irule no_err_eq_App_cong \\ fs [no_err_eq_refl]
-                \\ irule no_err_eq_Lam_cong \\ fs [])
-         \\ irule no_err_eq_trans \\ qexists_tac ‘Seq (Let v (Var n) (Projs ps (Var v))) (Let v (Var n) e)’
-         \\ conj_tac
-         THEN1 fs [Let_Seq]
-         \\ irule no_err_eq_Prim_cong
-         \\ fs [no_err_eq_refl]
-         \\ irule no_err_eq_trans \\ qexists_tac ‘Projs ps (Let v (Var n) (Var v))’
-         \\ conj_tac
-         THEN1 fs [Let_Projs]
-         \\ irule no_err_eq_Projs_cong \\ fs [Let_Var])
-  \\ qexists_tac ‘e’ \\ conj_tac
-  THEN1 fs [Let_Var_eq]
-  \\ irule no_err_eq_trans \\ qexists_tac ‘Seq (Projs ps (Var n)) e’
-  THEN1 fs []
-  \\ irule no_err_eq_Prim_cong \\ fs [no_err_eq_refl]
-QED
-
-Theorem fun_demands_Let:
-  ∀f. (f fun_demands (ps, k) ⇒ ∀e v. (App (Lam v f) e) fun_demands (ps, k))
-Proof
-  rw [fun_demands_def, Once fun_demands_pre_def, demands_def]
-  THEN1 (rw [fun_demands_pre_def]
-   \\ rw [demands_def]
-   \\ irule no_err_eq_trans \\ qexists_tac ‘Let v e (App f (Var n))’
-   \\ conj_tac
-   THEN1 (irule no_err_eq_trans \\ qexists_tac ‘App (Let v e f) (Let v e (Var n))’
-    \\ conj_tac
-    THEN1 (irule no_err_eq_App_cong \\ fs [no_err_eq_refl])
-*)
 
 Datatype:
   ctxt = Nil
-       | IsFree string ctxt
-       | Bind string exp ctxt ctxt
-       | RecBind ((string # exp) list) ctxt
-End
-
-Definition ctxt_size_def:
-  ctxt_size Nil = 0n ∧
-  ctxt_size (IsFree s ctxt) = 1 + ctxt_size ctxt ∧
-  ctxt_size (Bind s e ctxt tl) = 1 + list_size char_size s +  exp_size e + ctxt_size ctxt + ctxt_size tl ∧
-  ctxt_size (RecBind sel ctxt) = 1 + exp1_size sel + ctxt_size ctxt
-End
-
-Definition subst_ctxt_def:
-  (subst_ctxt ctxt (App f e) = App (subst_ctxt ctxt f) (subst_ctxt ctxt e)) ∧
-  (subst_ctxt  ctxt (Prim op l) = Prim op (MAP (subst_ctxt ctxt) l)) ∧
-  (subst_ctxt ctxt (Lam v e) = Lam v (subst_ctxt (IsFree v ctxt) e)) ∧
-  (subst_ctxt Nil (Var n) = Var n) ∧
-  (subst_ctxt (IsFree v ctxt) (Var n) = if n = v
-                                        then Var n
-                                        else subst_ctxt ctxt (Var n)) ∧
-  (subst_ctxt (Bind v exp ctxt tl) (Var n) = if n = v
-                                         then subst_ctxt ctxt exp
-                                         else subst_ctxt tl (Var n)) ∧
-  (subst_ctxt (RecBind nel ctxt) (Var n) = if MEM n (MAP FST nel)
-                                                then Var n
-                                                else subst_ctxt ctxt (Var n)) ∧
-  (subst_ctxt ctxt (Letrec nel e) = Letrec nel (subst_ctxt (RecBind nel ctxt) e))
-Termination
-  WF_REL_TAC ‘inv_image ($< LEX $<) (λ(c,e).(exp_size e + ctxt_size c, exp_size e))’
-  \\ rw [ctxt_size_def] \\ fs []
+       | Append ctxt ctxt
+       | Bind string exp ctxt
+       | RecBind (string # exp) ctxt
 End
 
 Inductive find: (* i i o o *)
 [find_Bottom:]
-  (∀e (c:ctxt).
+  (∀e c.
     find e c {} e) ∧
 [find_Seq:]
-  (∀e e' c (p:(string#num) list) ds v.
-    find e c ds e' ∧ (p,v) ∈ ds ⇒
-    find e c ds (Seq (Var v) e')) ∧
-[find_Seq2:]
-  (∀e e' e2 e2' c ds ds2.
-     find e c ds e' ∧ find e2 c ds2 e2' ⇒
-     find (Seq e e2) c ds (Seq e' e2')) ∧
-[find_If:]
-  (∀ec et ee ec' et' ee' c dsc dst dse.
-     find ec c dsc ec' ∧
-     find et c dst et' ∧
-     find ee c dse ee' ⇒
-     find (If ec et ee) c dsc (If ec' et' ee')) ∧
-[find_Var:]
-  (∀n c. find (Var n) c {([],n)} (Var n)) ∧
-[find_App:]
-  (∀f f' e e' c ds ds2.
-     find f c ds f' ∧
-     find e c ds2 e' ⇒
-     find (App f e) c ds (App f' e')) ∧
-[find_Prim:]
-  (∀c el el' ope.
-     LENGTH el = LENGTH el' ∧ (∀k. k < LENGTH el ⇒ ∃ds. find (EL k el) c ds (EL k el') )
-     ⇒ find (Prim ope el) c {} (Prim ope el')) ∧
-[find_Prim1:]
-  (∀c el el' ope ds.
-     LENGTH el = LENGTH el' ∧
-     (∀k. k < LENGTH el ⇒ ∃ds'. find (EL k el) c ds' (EL k el')) (* Rewritte with LIST_REL *)
-     ∧ find (EL 0 el) c ds (EL 0 el') ∧ el ≠ [] ∧ well_formed ope el ⇒ find (Prim ope el) c ds (Prim ope el')) ∧
-[find_Prim_Fail:]
-  (∀c el ope.
-     ¬ (well_written ope el) ⇒ find (Prim ope el) c {} Fail) ∧
-[find_Proj:]
-  (∀e e' n i c ds.
-     find e c ds e' ⇒ find (Proj n i e) c ds (Proj n i e')) ∧
-[find_IsEq:]
-  (∀e e' n i c ds.
-     find e c ds e' ⇒ find (IsEq n i e) c ds (IsEq n i e')) ∧
-[find_Subset:]
-  (∀e e' c ds ds'.
-     find e c ds e' ∧ (∀ps v. (ps, v) ∈ ds' ⇒ ∃ps'. (ps++ps', v) ∈ ds) ⇒ find e c ds' e') ∧
-[find_Let:]
-  (∀e e' e2 e2' ds ds' c v.
-     find e c ds e' ∧ find e2 (Bind v e c c) ds' e2'
-     ∧ (∀ps. (ps, v) ∉ ds')
-     ⇒ find (Let v e e2) c ds' (Let v e' e2')) ∧
-[find_Let2:]
-  (∀ e e' e2 e2' ds ds' ds'' c v ps.
-     find e c ds e' ∧ find e2 (Bind v e c c) ds' e2'
-     ∧ (ps,v) ∈ ds'
-     ∧ (∀ps' v'. (ps', v') ∈ ds'' ⇒ ((ps', v') ∈ ds' ∧ v' ≠ v) ∨ (ps', v') ∈ ds)
-     ⇒ find (Let v e e2) c ds'' (Let v e' e2')) ∧
-[find_Lam:]
-  (∀e e' c ds v.
-     find e c ds e' ⇒ find (Lam v e) c {} (Lam v e'))
+  (∀e c p ds v.
+    find e c ds e ∧ (p,v) ∈ ds ⇒
+    find e c ds (Seq (Var v) e))
 End
-
-
-fun apply_to_first_n 0 tac = ALL_TAC
-  | apply_to_first_n n tac = apply_to_first_n (n-1) tac >- tac;
-
-Theorem find_soundness_lemma:
-  ∀e c ds e'. find e c ds e'  ⇒
-                e no_err_rel e' ∧
-                (∀d. d ∈ ds ⇒ e demands d)
-Proof
-  Induct_on ‘find’
-  \\ rpt conj_tac
-  \\ rpt gen_tac
-  >- fs [no_err_eq_refl] (* find_Bottom *)
-  >~[‘e no_err_rel Seq (Var v) e2’] (* find_Seq *)
-  >- (strip_tac
-      \\ strip_tac
-      \\ fs []
-      \\ first_x_assum $ drule
-      \\ rw []
-      \\ dxrule_then assume_tac demands_empty_proj
-      \\ fs [demands_def, Projs_def]
-      \\ irule no_err_eq_trans
-      \\ first_assum $ irule_at Any
-      \\ irule no_err_eq_Prim_cong
-      \\ fs [no_err_eq_refl])
-  >~[‘Seq e e2 no_err_rel Seq e' e2'’] (* find_Seq2 *)
-  >- (rw []
-      \\ fs [no_err_eq_Prim_cong, demands_Seq])
-  >~[‘If ec et ee no_err_rel If ec' et' ee'’]
-  >- (rw []
-      \\ fs [demands_If, no_err_eq_Prim_cong])
-  >~[‘Var n no_err_rel Var n’] (* find_Var *)
-  >- fs [no_err_eq_refl, demands_Var]
-  >~[‘App f e no_err_rel App f' e'’] (* find_App *)
-  >- (rw []
-      \\ fs [no_err_eq_App_cong, demands_App])
-  >~[‘Proj n i e no_err_rel Proj n i e'’] (* find_Proj *)
-  >- (strip_tac
-      \\ fs [no_err_eq_Prim_cong, demands_Proj])
-  >~[‘IsEq n i e no_err_rel IsEq n i e'’] (* find_IsEq *)
-  >- (rw []
-      \\ fs [no_err_eq_Prim_cong, demands_IsEq])
-  >>~[‘Prim ope el1 no_err_rel Prim ope el2’] (* find_Prim *)
-  >- (rw []
-      \\ irule no_err_eq_Prim_cong
-      \\ rw [LIST_REL_EL_EQN, EL_MAP]
-      \\ rename1 ‘EL n _’
-      \\ ‘n < LENGTH el1’ by fs []
-      \\ first_x_assum drule
-      \\ rw [])
-  >- (rw [] (* find_Prim1 *)
-      >- (irule no_err_eq_Prim_cong
-          \\ rw [LIST_REL_EL_EQN, EL_MAP]
-          \\ rename1 ‘EL n _’
-          \\ ‘n < LENGTH el1’ by fs []
-          \\ first_x_assum drule
-          \\ rw []
-          \\ fs [])
-      \\ rw []
-      \\ last_x_assum dxrule
-      \\ rw []
-      \\ Cases_on ‘el1’
-      \\ fs [demands_Prim])
-  >~[‘Prim ope el1 no_err_rel Fail’] (* find_Prim_Fail *)
-  >- (rw []
-      \\ fs [not_well_written_is_fail])
-  >>~[‘Let v e e2 no_err_rel Let v e' e2'’] (* find_Let *)
-  >- (rw []
-      \\ fs [no_err_eq_App_cong, no_err_eq_Lam_cong]
-      \\ rename1 ‘_ demands d’
-      \\ PairCases_on ‘d’
-      \\ irule demands_Let2
-      \\ ‘d1 = v ∨ d1 ≠ v’ by fs []
-      \\ fs []
-      \\ last_x_assum irule
-      \\ first_x_assum $ irule_at Any)
-  >- (rw []
-      \\ fs [no_err_eq_App_cong, no_err_eq_Lam_cong]
-      \\ rename1 ‘_ demands d’
-      \\ PairCases_on ‘d’
-      \\ first_x_assum dxrule
-      \\ rw []
-      >- fs [demands_Let2]
-      \\ irule demands_Let1
-      \\ fs []
-      \\ first_x_assum drule
-      \\ rw []
-      \\ drule demands_empty_proj
-      \\ fs [])
-  >- (rw [] (* find_Subset *)
-      \\ rename1 ‘e demands d’ \\ PairCases_on ‘d’
-      \\ first_x_assum drule
-      \\ rw []
-      \\ first_x_assum drule
-      \\ rw []
-      \\ drule demands_projs_reduce
-      \\ fs [])
-  >- (rw [] (* find_Lam *)
-      \\ fs [no_err_eq_Lam_cong])
-QED
-
-Theorem find_soundness:
-  find e Nil ds e' ⇒ e no_err_rel e'
-Proof
-  rw []
-  \\ dxrule find_soundness_lemma
-  \\ fs []
-QED
-
-Datatype:
-  demands_tree = DemandNode bool (((string # num) # demands_tree) list)
-End
-
-Definition dt_to_set_def:
-  dt_to_set (DemandNode T []) ps v = {(ps,v)} ∧
-  dt_to_set (DemandNode F []) ps v = {} ∧
-  dt_to_set (DemandNode b ((p, dt)::tl)) ps v = (dt_to_set dt (ps ++ [p]) v) ∪ (dt_to_set (DemandNode b tl) ps v)
-End
-
-Definition merge_dt_def:
-  merge_dt (DemandNode b1 f1) (DemandNode b2 []) = DemandNode (b1 ∨ b2) f1 ∧
-  merge_dt (DemandNode b1 []) (DemandNode b2 f2) = DemandNode (b1 ∨ b2) f2 ∧
-  merge_dt (DemandNode b1 ((id1,dt1)::tl1)) (DemandNode b2 ((id2,dt2)::tl2)) =
-  if id1 = id2
-  then
-    case merge_dt (DemandNode b1 tl1) (DemandNode b2 tl2) of
-    | DemandNode b3 tl3 => DemandNode b3 ((id1, merge_dt dt1 dt2)::tl3) (* id1 = id2 *)
-  else
-    if FST id1 < FST id2 ∨ (FST id1 = FST id2 ∧ SND id1 < SND id2)
-    then
-      case merge_dt (DemandNode b1 tl1) (DemandNode b2 ((id2,dt2)::tl2)) of
-      | DemandNode b3 tl3 => DemandNode b3 ((id1, dt1)::tl3) (* id1 < id2 *)
-    else
-      case merge_dt (DemandNode b1 ((id1,dt1)::tl1)) (DemandNode b2 tl2) of
-      | DemandNode b3 tl3 => DemandNode b3 ((id2, dt2)::tl3) (* id2 < id1 *)
-End
-
-Definition find_function_def:
-  find_function (Var v) c = ((FEMPTY : (string |-> demands_tree)) |+ (v, DemandNode T []), Var v) ∧
-  (find_function (If ce te ee) c =
-   let (cd, ce') = find_function ce c in
-     let (td, te') = find_function te c in
-       let (ed, ee') = find_function ee c in
-         (cd, If ce' te' ee')) ∧
-  (find_function (Prim If _) c = (FEMPTY, Fail)) ∧
-  (find_function (Proj s i e) c =
-   let (d, e') = find_function e c in
-     (d, Proj s i e')) ∧
-  (find_function (Prim (Proj s i) _) c = (FEMPTY, Fail)) ∧
-  (find_function (IsEq s i e) c =
-   let (d, e') = find_function e c in
-     (d, IsEq s i e')) ∧
-  (find_function (Prim (IsEq s i) _) c = (FEMPTY, Fail)) ∧
-  (find_function (Seq e1 e2) c =
-   let (d1, e1') = find_function e1 c in
-     let (d2, e2') = find_function e2 c in
-       (d1, Seq e1' e2')) ∧
-  (find_function (Prim Seq _) c = (FEMPTY, Fail)) ∧
-  (find_function (Prim op l) c =
-  (FEMPTY, Prim op (MAP (λe. SND (find_function e c)) l))) ∧
-  (find_function (App (Lam v e2) e) c = let (d, e') = find_function e c in
-                                          let (d2, e2') = find_function e2 (Bind v e c c) in
-                                           case FLOOKUP d2 v of
-                                             | NONE => (d2, App (Lam v e2') e')
-                                             | SOME s => (FMERGE merge_dt d (d2 \\ v), Let v e' (Seq (Var v) e2'))) ∧
-  (find_function (App f e) c = let (d, f') = find_function f c in
-                                 let (_, e') = find_function e c in
-                                   (d, App f' e')) ∧
-  find_function e c = ((FEMPTY, e) : (string |-> demands_tree) # exp)
-Termination
-  WF_REL_TAC ‘measure (exp_size o FST)’
-  \\ rw [] \\ fs []
-  \\ assume_tac exp_size_lemma
-  \\ fs []
-  \\ first_x_assum dxrule
-  \\ fs []
-End
-
-Theorem exp_size_cmp_exp3_size:
-  ∀l e. MEM e l ⇒ exp_size e < exp3_size l
-Proof
-  fs [exp_size_lemma]
-QED
-
-Definition demands_tree_size_def:
-  demands_tree_size (DemandNode b []) = 1 ∧
-  demands_tree_size (DemandNode b ((v,dt)::tl)) = 1 + demands_tree_size dt + demands_tree_size (DemandNode b tl)
-End
-
-Theorem dt_to_set_union:
-  ∀l b p v. dt_to_set (DemandNode T l) p v = {(p, v)} ∪ dt_to_set (DemandNode b l) p v
-Proof
-  Induct
-  \\ rw [dt_to_set_def]
-  >- (rename1 ‘DemandNode b []’
-      \\ Cases_on ‘b’
-      \\ rw [dt_to_set_def])
-  \\ rename1 ‘DemandNode b (hd::tl)’
-  \\ Cases_on ‘hd’
-  \\ rw [dt_to_set_def]
-  \\ metis_tac [UNION_COMM, UNION_ASSOC]
-QED
-
-Theorem merge_dt_is_set_union:
-  ∀dt1 dt2 p v. dt_to_set (merge_dt dt1 dt2) p v = (dt_to_set dt1 p v) ∪ (dt_to_set dt2 p v)
-Proof
-  Induct using demands_tree_size_ind
-  >- (Cases
-      \\ Cases
-      \\ rename1 ‘DemandNode b2 l’
-      \\ Cases_on ‘b2’
-      \\ Cases_on ‘l’
-      \\ rw [merge_dt_def, dt_to_set_def]
-      \\ fs [dt_to_set_union])
-  \\ Induct using demands_tree_size_ind
-  >- (rpt gen_tac
-      \\ rename1 ‘DemandNode b2 []’
-      \\ Cases_on ‘b2’
-      \\ rw [dt_to_set_def, merge_dt_def]
-      \\ metis_tac [dt_to_set_union, UNION_COMM, UNION_ASSOC])
-  \\ rpt gen_tac
-  \\ rename1 ‘merge_dt (DemandNode b1 ((v1,dt1)::tl1)) (DemandNode b2 ((v2,dt2)::tl2))’
-  \\ rw [merge_dt_def]
-  >- (qabbrev_tac ‘dt3 = merge_dt (DemandNode b1 tl1) (DemandNode b2 tl2)’
-      \\ Cases_on ‘dt3’
-      \\ rw [dt_to_set_def]
-      \\ unabbrev_all_tac
-      \\ metis_tac [UNION_COMM, UNION_ASSOC])
-  >- (qabbrev_tac ‘dt3 = merge_dt (DemandNode b1 tl1) (DemandNode b2 ((v2,dt2)::tl2))’
-      \\ Cases_on ‘dt3’
-      \\ rw [dt_to_set_def]
-      \\ unabbrev_all_tac
-      \\ metis_tac [UNION_COMM, UNION_ASSOC, dt_to_set_def])
-  >- (qabbrev_tac ‘dt3 = merge_dt (DemandNode b1 tl1) (DemandNode b2 ((v2,dt2)::tl2))’
-      \\ Cases_on ‘dt3’
-      \\ rw [dt_to_set_def]
-      \\ unabbrev_all_tac
-      \\ metis_tac [UNION_COMM, UNION_ASSOC, dt_to_set_def])
-  \\ qabbrev_tac ‘dt3 = merge_dt (DemandNode b1 ((v1, dt1)::tl1)) (DemandNode b2 tl2)’
-  \\ Cases_on ‘dt3’
-  \\ rw [dt_to_set_def]
-  \\ unabbrev_all_tac
-  \\ metis_tac [UNION_COMM, UNION_ASSOC]
-QED
-
-Theorem find_function_soundness_lemma:
-  ∀k e c d e' b.
-    exp_size e < k ⇒
-    find_function e c = (d, e') ⇒
-    ∃ds. find e c ds e' ∧
-         (∀s ps. (ps, s) ∈ ds ⇒ ∃dt. FLOOKUP d s = SOME dt ∧ (ps, s) ∈ dt_to_set dt [] s) ∧
-         (∀s. s ∈ FDOM d ⇒ ∃ps. (ps, s) ∈ ds)
-Proof
-  Induct (* completeInduct_on ‘exp_size e’ *)
-  \\ gen_tac \\ Cases_on ‘e’
-  \\ fs [exp_size_def]
-  >- (rw [find_function_def] (* Var v *)
-      \\ rename1 ‘(v, DemandNode T [])’
-      \\ qexists_tac ‘{([], v)}’
-      \\ fs [find_Var]
-      \\ qexists_tac ‘DemandNode T []’
-      \\ rw [dt_to_set_def, FLOOKUP_UPDATE])
-  >- (rw [] (* Prim op l *)
-      \\ rename1 ‘Prim op es’
-      \\ Cases_on ‘es’
-      >- (Cases_on ‘op’ (* Prim op [] *)
-          \\ fs [find_function_def]
-          \\ qexists_tac ‘{}’
-          \\ fs [find_Bottom]
-          \\ irule find_Prim_Fail
-          \\ fs [well_written_def])
-      \\ rename1 ‘h::t’
-      \\ Cases_on ‘op’ >~[‘Prim (Cons s) (h::tl)’]
-      >- (fs [find_function_def]
-          \\ qabbrev_tac ‘es = h::tl’
-          \\ qexists_tac ‘{}’
-          \\ fs []
-          \\ rw []
-          \\ irule find_Prim
-          \\ rw [] >~[‘LENGTH _ = _’] >- (unabbrev_all_tac \\ fs [])
-          \\ rename1 ‘EL k' es’
-          \\ ‘exp_size (EL k' es) < k’ by
-            (‘exp_size (EL k' es) < exp3_size es’ by
-               (irule exp_size_cmp_exp3_size
-                \\ fs [MEM_EL]
-                \\ qexists_tac ‘k'’
-                \\ fs []
-                \\ unabbrev_all_tac
-                \\ fs [])
-             \\ fs [])
-          \\ first_x_assum dxrule
-          \\ qabbrev_tac ‘de = find_function (EL k' es) c’
-          \\ PairCases_on ‘de’
-          \\ rw []
-          \\ ‘de1 = EL k' (MAP (λe. SND (find_function e c)) es)’ by
-            fs [EL_MAP]
-          \\ fs[]
-          \\ unabbrev_all_tac
-          \\ fs []
-          \\ first_x_assum drule
-          \\ rw []
-          \\ first_x_assum $ irule_at Any)
-      >- (Cases_on ‘t’
-          >- (fs [find_function_def] (* Prim If [e] *)
-              \\ qexists_tac ‘{}’
-              \\ fs []
-              \\ rw []
-              \\ fs [find_Prim_Fail, well_written_def])
-          \\ rename1 ‘h::h1::t’
-          \\ Cases_on ‘t’
-          >- (fs [find_function_def] (* Prim If [e, e'] *)
-              \\ qexists_tac ‘{}’
-              \\ rw []
-              \\ fs [find_Prim_Fail, well_written_def])
-          \\ rename1 ‘ce::te::ee::t’
-          \\ Cases_on ‘t’
-          >- (fs [find_function_def] (* If _ _ _ *)
-              \\ qabbrev_tac ‘ce' = find_function ce c’ \\ PairCases_on ‘ce'’
-              \\ qabbrev_tac ‘te' = find_function te c’ \\ PairCases_on ‘te'’
-              \\ qabbrev_tac ‘ee' = find_function ee c’ \\ PairCases_on ‘ee'’
-              \\ fs []
-              \\ ‘exp_size ce < k’ by fs [exp_size_def]
-              \\ first_assum dxrule
-              \\ ‘exp_size te < k’ by fs [exp_size_def]
-              \\ first_assum dxrule
-              \\ ‘exp_size ee < k’ by fs [exp_size_def]
-              \\ first_x_assum dxrule
-              \\ rw []
-              \\ first_x_assum dxrule
-              \\ rw []
-              \\ rename1 ‘find ce c ds ce'1’
-              \\ first_x_assum dxrule
-              \\ first_x_assum dxrule
-              \\ rw []
-              \\ qexists_tac ‘ds’
-              \\ fs []
-              \\ irule find_If
-              \\ fs []
-              \\ conj_tac
-              \\ first_x_assum $ irule_at Any)
-          \\ fs [find_function_def]
-          \\ qexists_tac ‘{}’
-          \\ rw []
-          \\ fs [find_Prim_Fail, well_written_def])
-      >- (Cases_on ‘t’ (* IsEq *)
-          \\ fs [find_function_def]
-          >- (qabbrev_tac ‘ff = find_function h c’
-              \\ PairCases_on ‘ff’
-              \\ ‘exp_size h < k’ by fs [exp_size_def]
-              \\ first_x_assum dxrule
-              \\ rw []
-              \\ fs []
-              \\ first_x_assum drule
-              \\ rw []
-              \\ qexists_tac ‘ds’
-              \\ fs []
-              \\ fs [find_IsEq])
-          \\ qexists_tac ‘{}’
-          \\ fs [find_Prim_Fail, well_written_def])
-      >- (Cases_on ‘t’ (* Proj *)
-          \\ fs [find_function_def]
-          >- (qabbrev_tac ‘ff = find_function h c’
-              \\ PairCases_on ‘ff’
-              \\ ‘exp_size h < k’ by fs [exp_size_def]
-              \\ first_x_assum dxrule
-              \\ rw []
-              \\ fs []
-              \\ first_x_assum drule
-              \\ rw []
-              \\ qexists_tac ‘ds’
-              \\ fs []
-              \\ irule find_Proj
-              \\ first_assum $ irule_at Any)
-          \\ qexists_tac ‘{}’
-          \\ fs [find_Prim_Fail, well_written_def])
-      >- (qabbrev_tac ‘l = h::t’ (* AtomOp *)
-         \\ qexists_tac ‘{}’
-         \\ fs [find_function_def]
-         \\ rw []
-         \\ irule find_Prim
-         \\ rw []
-         \\ rename1 ‘n < LENGTH l’
-         \\ ‘exp_size (EL n l) < k’ by
-           (‘exp_size (EL n l) < exp3_size l’ by fs [exp_size_cmp_exp3_size, EL_MEM]
-           \\ fs [])
-          \\ first_x_assum dxrule
-          \\ rw []
-          \\ qabbrev_tac ‘triple = find_function (EL n l) c’
-          \\ PairCases_on ‘triple’
-          \\ fs []
-          \\ first_x_assum drule
-          \\ rw [EL_MAP]
-          \\ first_x_assum $ irule_at Any)
-      >- (Cases_on ‘t’ (* Seq *)
-          >- (fs [find_function_def]
-              \\ qexists_tac ‘{}’
-              \\ fs [find_Prim_Fail, well_written_def])
-          \\ rename1 ‘h0::h1::tl’
-          \\ Cases_on ‘tl’
-          >- (‘exp_size h0 < k’ by fs [exp_size_def]
-              \\ first_assum dxrule
-              \\ ‘exp_size h1 < k’ by fs [exp_size_def]
-              \\ first_x_assum dxrule
-              \\ rw []
-              \\ fs [find_function_def]
-              \\ qabbrev_tac ‘f1 = find_function h1 c’
-              \\ PairCases_on ‘f1’
-              \\ qabbrev_tac ‘f0 = find_function h0 c’
-              \\ PairCases_on ‘f0’
-              \\ fs []
-              \\ first_x_assum drule
-              \\ first_x_assum drule
-              \\ rw []
-              \\ qexists_tac ‘ds'’
-              \\ fs []
-              \\ irule find_Seq2
-              \\ fs []
-              \\ first_x_assum $ irule_at Any)
-          \\ fs [find_function_def]
-          \\ qexists_tac ‘{}’
-          \\ fs [find_Prim_Fail, well_written_def]))
-  >- (rw [] (* App *)
-      \\ rename1 ‘App f e’
-      \\ ‘exp_size f < k’ by fs []
-      \\ first_assum dxrule
-      \\ qabbrev_tac ‘e1p = find_function f c’
-      \\ PairCases_on ‘e1p’
-      \\ strip_tac
-      \\ fs []
-      \\ first_x_assum drule
-      \\ strip_tac
-      \\ Cases_on ‘f’ >~[‘Let s e e2’]
-      >- (
-       fs [find_function_def]
-       \\ qabbrev_tac ‘ep = find_function e c’
-       \\ PairCases_on ‘ep’
-       \\ qabbrev_tac ‘e2p = find_function e2 (Bind s e c c)’
-       \\ PairCases_on ‘e2p’
-       \\ fs []
-       \\ ‘exp_size e < k’ by fs []
-       \\ first_assum dxrule
-       \\ ‘exp_size e2 < k’ by
-         (‘exp_size e2 < exp_size (Lam s e2)’ by fs [exp_size_def]
-          \\ rw [] \\ fs [])
-       \\ first_x_assum dxrule
-       \\ rw []
-       \\ first_x_assum drule
-       \\ first_x_assum drule
-       \\ rw []
-       \\ ‘s ∈ FDOM e2p0 ∨ s ∉ FDOM e2p0’ by fs []
-       \\ fs [FLOOKUP_DEF]
-       \\ rw []
-       >- (
-         ‘∃ds'''. ∀ps v. (ps, v) ∈ ds''' ⇔ ((ps, v) ∈ ds' ∧ v ≠ s) ∨ (ps, v) ∈ ds''’ by
-            (qexists_tac ‘ds'' ∪ BIGUNION (IMAGE (λ(ps,v). if v = s then {} else {(ps,v)}) ds')’
-             \\ rw []
-             \\ eq_tac
-             \\ rw []
-             \\ fs []
-             >- (rename1 ‘p ∈ ds'’
-                 \\ PairCases_on ‘p’
-                 \\ fs []
-                 \\ ‘p1 = s ∨ p1 ≠ s’ by fs []
-                 \\ fs [])
-             \\ rw [DISJ_EQ_IMP]
-             \\ qexists_tac ‘{(ps, v)}’
-             \\ fs []
-             \\ first_x_assum $ irule_at Any
-             \\ fs [])
-         \\ irule_at Any find_Let2
-         \\ first_assum $ irule_at Any
-         \\ last_assum dxrule
-         \\ rw []
-         \\ first_assum $ irule_at Any
-         \\ irule_at Any find_Seq
-         \\ first_assum $ irule_at Any
-         \\ qexists_tac ‘ds'''’
-         \\ fs []
-         \\ rw []
-         >- (first_assum dxrule
-             \\ first_x_assum dxrule
-             \\ fs [])
-         >- (rw [FMERGE_DEF]
-             >- (first_assum dxrule
-                 \\ first_x_assum dxrule
-                 \\ rw []
-                 \\ qsuff_tac ‘FLOOKUP (e2p0 \\ s) s' = FLOOKUP e2p0 s'’
-                 >- rw [FLOOKUP_DEF]
-                 \\ fs [DOMSUB_FLOOKUP_NEQ])
-             >- (last_assum dxrule
-                 \\ last_x_assum dxrule
-                 \\ fs [])
-             \\ last_assum dxrule
-             \\ last_assum dxrule
-             \\ rw [merge_dt_is_set_union]
-             \\ qsuff_tac ‘FLOOKUP (e2p0 \\ s) s' = FLOOKUP e2p0 s'’
-             >- rw [FLOOKUP_DEF]
-             \\ fs [DOMSUB_FLOOKUP_NEQ])
-         >- (first_x_assum dxrule
-             \\ first_x_assum dxrule
-             \\ fs [])
-         >- (first_x_assum dxrule
-             \\ rw [FMERGE_DEF, merge_dt_is_set_union])
-         >- (first_x_assum dxrule
-             \\ rw []
-             \\ qexists_tac ‘ps'’
-             \\ fs [])
-         \\ first_x_assum dxrule
-         \\ rw []
-         \\ qexists_tac ‘ps'’
-         \\ fs [])
-       \\ irule_at Any find_Let
-       \\ last_x_assum $ irule_at Any
-       \\ last_x_assum $ irule_at Any
-       \\ fs []
-       \\ rw []
-       >- (strip_tac
-           \\ first_x_assum dxrule
-           \\ fs [])
-       \\ first_assum drule
-       \\ fs [])
-      \\ fs [find_function_def]
-      \\ ‘exp_size e < k’ by fs []
-      \\ first_x_assum dxrule
-      \\ rw []
-      \\ qabbrev_tac ‘ep = find_function e c’
-      \\ PairCases_on ‘ep’
-      \\ fs []
-      \\ first_x_assum drule
-      \\ rw []
-      \\ irule_at Any find_App
-      \\ first_assum $ irule_at Any >~[‘Var s’]
-      >- (irule_at Any find_Var
-          \\ qexists_tac ‘[]’
-          \\ fs []
-          \\ rw [FLOOKUP_UPDATE, dt_to_set_def])
-      \\ first_assum $ irule_at Any
-      \\ fs [])
-  >- (rw [find_function_def] (* Lam *)
-      \\ irule_at Any find_Bottom
-      \\ fs [])
-  >- (rw [find_function_def] (* Letrec *)
-      \\ irule_at Any find_Bottom
-      \\ fs [find_Bottom])
-QED
-
-
-Definition demand_analysis_def:
-  demand_analysis = SND o (λe. find_function e Nil)
-End
-
-Theorem demand_analysis_soundness:
-  ∀e. is_closed e ⇒ e no_err_rel demand_analysis e
-Proof
-  rw [demand_analysis_def]
-  \\ qabbrev_tac ‘p = find_function e Nil’
-  \\ PairCases_on ‘p’
-  \\ fs []
-  \\ irule find_soundness
-  \\ ‘exp_size e < SUC (exp_size e)’ by fs []
-  \\ drule find_function_soundness_lemma
-  \\ rw []
-  \\ first_x_assum dxrule
-  \\ rw []
-  \\ first_assum $ irule_at Any
-QED
 
 (*
+
   let foo = lam (a + 2) in
     lam x (foo x)
 -->
@@ -1309,6 +217,7 @@ QED
     lam x (seq x (foo x))
 
   Letrec [(f,x)] rest
+
 *)
 
 val _ = export_theory();
