typing/pure_inferenceScript.sml
@@ -1,0 +1,622 @@
+(*
+  Type inference in the style of:
+  "Generalizing Hindley-Milner Type Inference Algorithms" by Heeren et al.
+  (http://www.cs.uu.nl/research/techreps/repo/CS-2002/2002-031.pdf)
+
+  Other resources include
+  - https://www.researchgate.net/profile/Martin-Sulzmann/publication/2802561_HindleyMilner_[…]0/Hindley-Milner-style-type-systems-in-constraint-form.pdf
+  - http://gallium.inria.fr/~fpottier/publis/emlti-final.pdf
+*)
+open HolKernel Parse boolLib bossLib BasicProvers dep_rewrite;
+open pairTheory arithmeticTheory integerTheory stringTheory optionTheory
+     listTheory alistTheory finite_mapTheory sptreeTheory monadsyntax;
+open pure_typingTheory pure_cexpTheory pure_configTheory pure_varsTheory
+     pure_inference_commonTheory pure_unificationTheory pure_miscTheory;
+
+val _ = new_theory "pure_inference";
+
+
+(******************** Inference monad ********************)
+(*
+  For now this is just a state/error monad.
+  The state (a number) keeps track of the next fresh variable.
+
+  TODO make return type a sum, with some basic errors:
+    unbound variable
+    incorrect arity (e.g. supplying arguments to Lit, nullary functions, ...)
+
+  Some of these errors will be picked up by the parser, but still should be
+  handled gracefully.
+*)
+Type inferM[pp] = ``:num -> ('a # num) option``
+
+Definition infer_bind_def:
+  infer_bind (g : 'a inferM) f s =
+    case g s of
+    | NONE => NONE
+    | SOME (x, s') => (f x : 'b inferM) s'
+End
+
+Definition infer_ignore_bind_def:
+  infer_ignore_bind g f = infer_bind g (λ_ s. f s)
+End
+
+Definition return_def:
+  return x =  λs. SOME (x, s)
+End
+
+Definition fail_def:
+  fail : 'a inferM = λs. NONE
+End
+
+val infer_monadinfo : monadinfo = {
+  bind = “infer_bind”,
+  ignorebind = SOME “infer_ignore_bind”,
+  unit = “return”,
+  fail = SOME “fail”,
+  choice = NONE,
+  guard = NONE
+  };
+
+val _ = declare_monad ("infer", infer_monadinfo);
+val _ = enable_monadsyntax ();
+val _ = enable_monad "infer";
+
+(********** Key monadic helpers **********)
+
+Definition oreturn_def:
+  oreturn NONE = fail ∧
+  oreturn (SOME x) = return x
+End
+
+Definition fresh_var_def:
+  fresh_var : num inferM = λs. SOME (s, SUC s)
+End
+
+Definition fresh_vars_def:
+  fresh_vars vars : num list inferM =
+    λs. SOME (GENLIST (λn:num. s + n) vars, s + vars)
+End
+
+
+(******************** Constraint types ********************)
+
+Datatype:
+  constraint = Unify 'a itype itype
+             | Instantiate 'a itype (num # itype)
+             | Implicit 'a itype (num_set) itype
+End
+
+Type assumptions[pp] = ``:num_set var_map``;
+
+Definition aunion_def:
+  aunion = unionWith sptree$union : assumptions -> assumptions -> assumptions
+End
+
+val _ = set_mapped_fixity {term_name = "aunion", tok = UTF8.chr 0x22D3,
+                           fixity = Infixl 500}
+
+Definition get_assumptions_def:
+  get_assumptions var (assumptions : assumptions) =
+    case lookup assumptions var of
+    | NONE => []
+    | SOME cvars => MAP FST $ toAList cvars
+End
+
+Definition singleton_def:
+  singleton k v = insert empty k v
+End
+
+
+(******************** Constraint generation ********************)
+
+Definition infer_cons_def:
+  infer_cons n ([] : typedefs) cname = NONE ∧
+  infer_cons n ((ar,cs)::tds) cname =
+    case ALOOKUP cs cname of
+    | SOME ts => SOME (n, ar, ts)
+    | NONE => infer_cons (SUC n) tds cname
+End
+
+(*
+  We include arity as an argument to handle the fact that
+  Substring/Concat/Implode separately have multiple possible arities.
+*)
+Definition infer_atom_op_def:
+  (infer_atom_op ar (Lit $ Int i) =
+    if ar = 0n then SOME ([], Integer) else NONE) ∧
+  (infer_atom_op ar (Lit $ Str s) =
+    if ar = 0 then SOME ([], String) else NONE) ∧
+  (infer_atom_op ar (Lit $ Msg s1 s2) =
+    if ar = 0 then SOME ([], Message) else NONE) ∧
+  (infer_atom_op ar (Lit $ Loc n) = NONE) ∧
+  (infer_atom_op ar Add =
+    if ar = 2 then SOME ([Integer; Integer], Integer) else NONE) ∧
+  (infer_atom_op ar Sub =
+    if ar = 2 then SOME ([Integer; Integer], Integer) else NONE) ∧
+  (infer_atom_op ar Mul =
+    if ar = 2 then SOME ([Integer; Integer], Integer) else NONE) ∧
+  (infer_atom_op ar Div =
+    if ar = 2 then SOME ([Integer; Integer], Integer) else NONE) ∧
+  (infer_atom_op ar Mod =
+    if ar = 2 then SOME ([Integer; Integer], Integer) else NONE) ∧
+  (infer_atom_op ar Eq =
+    if ar = 2 then SOME ([Integer; Integer], Bool) else NONE) ∧
+  (infer_atom_op ar Lt =
+    if ar = 2 then SOME ([Integer; Integer], Bool) else NONE) ∧
+  (infer_atom_op ar Leq =
+    if ar = 2 then SOME ([Integer; Integer], Bool) else NONE) ∧
+  (infer_atom_op ar Gt =
+    if ar = 2 then SOME ([Integer; Integer], Bool) else NONE) ∧
+  (infer_atom_op ar Geq =
+    if ar = 2 then SOME ([Integer; Integer], Bool) else NONE) ∧
+  (infer_atom_op ar Len =
+    if ar = 1 then SOME ([String], Integer) else NONE) ∧
+  (infer_atom_op ar Elem =
+    if ar = 2 then SOME ([String; Integer], Integer) else NONE) ∧
+  (infer_atom_op ar Concat = SOME (REPLICATE ar String, String)) ∧
+  (infer_atom_op ar Implode = SOME (REPLICATE ar Integer, String)) ∧
+  (infer_atom_op ar Substring =
+    if ar = 2 then SOME ([String; Integer], String)
+    else if ar = 3 then SOME ([String; Integer; Integer], String) else NONE) ∧
+  (infer_atom_op ar StrEq =
+    if ar = 2 then SOME ([String; String], Bool) else NONE) ∧
+  (infer_atom_op ar StrLt =
+    if ar = 2 then SOME ([String; String], Bool) else NONE) ∧
+  (infer_atom_op ar StrLeq =
+    if ar = 2 then SOME ([String; String], Bool) else NONE) ∧
+  (infer_atom_op ar StrGt =
+    if ar = 2 then SOME ([String; String], Bool) else NONE) ∧
+  (infer_atom_op ar StrGeq =
+    if ar = 2 then SOME ([String; String], Bool) else NONE) ∧
+  (infer_atom_op ar (Message s) =
+    if ar = 1 then SOME ([String], Message : prim_ty) else NONE)
+End
+
+Definition get_typedef_def:
+  get_typedef n ([] : typedefs) cnames_arities = NONE ∧
+  get_typedef n ((ar,cs)::tds) cnames_arities =
+    if
+      LENGTH cs = LENGTH cnames_arities ∧
+      EVERY (λ(cn,ts). MEM (cn, LENGTH ts) cnames_arities) cs
+    then SOME (n, ar, cs)
+    else get_typedef (SUC n) tds cnames_arities
+End
+
+(**********
+  infer :
+       exndef # typedefs -- type definitions for exceptions and datatypes
+    -> cexp -> (itype, assumptions, constraint list) inferM
+**********)
+Definition infer_def:
+  infer (ns : exndef # typedefs) mset (pure_cexp$Var d x) = do
+    fresh <- fresh_var;
+    return (CVar fresh, singleton x (insert fresh () LN), []) od ∧
+
+  infer ns mset (Prim d (Cons s) es) = (
+    if s = "" then do
+      (tys,as,cs) <- FOLDR
+            (λe acc. do
+                (tys, as, cs) <- acc;
+                (ty, as', cs') <- infer ns mset e;
+                return (ty::tys, as ⋓ as', cs' ++ cs) od)
+            (return ([],empty,[])) es;
+      return (Tuple tys, as, cs) od
+
+    else if s = "Ret" then (
+      case es of
+      | [e] => do (ty, as, cs) <- infer ns mset e; return (M ty, as, cs) od
+      | _ => fail)
+
+    else if s = "Bind" then (
+      case es of
+      | [e1; e2] => do
+          (ty2, as2, cs2) <- infer ns mset e2;
+          (ty1, as1, cs1) <- infer ns mset e1;
+          fresh1 <- fresh_var; fresh2 <- fresh_var;
+          return
+            (M $ CVar fresh2, as1 ⋓ as2,
+             (Unify d ty1 $ M $ CVar fresh1)::
+              (Unify d ty2 $ Function (CVar fresh1) (M $ CVar fresh2))::(cs1++cs2))
+          od
+      | _ => fail)
+
+    else if s = "Raise" then (
+      case es of
+      | [e] => do
+          (ty, as, cs) <- infer ns mset e;
+          fresh <- fresh_var;
+          return (M $ CVar fresh, as,
+            (Unify d (CVar fresh) (CVar fresh))::(Unify d ty Exception)::cs) od
+      | _ => fail)
+
+    else if s = "Handle" then (
+      case es of
+      | [e1; e2] => do
+          (ty2, as2, cs2) <- infer ns mset e2;
+          (ty1, as1, cs1) <- infer ns mset e1;
+          fresh <- fresh_var;
+          return
+            (M $ CVar fresh, as1 ⋓ as2,
+             (Unify d ty1 $ M $ CVar fresh)::
+              (Unify d ty2 $ Function Exception (M $ CVar fresh))::(cs1++cs2))
+          od
+      | _ => fail)
+
+    else if s = "Act" then (
+      case es of
+      | [e] => do
+          (ty, as, cs) <- infer ns mset e;
+          return (M $ PrimTy String, as, (Unify d ty $ PrimTy Message)::cs) od
+      | _ => fail)
+
+    else if s = "Alloc" then (
+      case es of
+      | [e1; e2] => do
+          (ty2, as2, cs2) <- infer ns mset e2;
+          (ty1, as1, cs1) <- infer ns mset e1;
+          return
+            (M $ Array ty2, as1 ⋓ as2, (Unify d ty1 $ PrimTy Integer)::(cs1++cs2))
+          od
+      | _ => fail)
+
+    else if s = "Length" then (
+      case es of
+      | [e] => do
+          (ty, as, cs) <- infer ns mset e;
+          fresh <- fresh_var;
+          return
+            (M $ PrimTy Integer, as, (Unify d ty $ Array $ CVar fresh)::cs)
+          od
+      | _ => fail)
+
+    else if s = "Deref" then (
+      case es of
+      | [e1; e2] => do
+          (ty2, as2, cs2) <- infer ns mset e2;
+          (ty1, as1, cs1) <- infer ns mset e1;
+          fresh <- fresh_var;
+          return
+            (M $ CVar fresh, as1 ⋓ as2,
+              (Unify d ty2 $ PrimTy Integer)::
+              (Unify d ty1 $ Array $ CVar fresh)::(cs1++cs2))
+          od
+      | _ => fail)
+
+    else if s = "Update" then (
+      case es of
+      | [e1; e2; e3] => do
+          (ty3, as3, cs3) <- infer ns mset e3;
+          (ty2, as2, cs2) <- infer ns mset e2;
+          (ty1, as1, cs1) <- infer ns mset e1;
+          fresh <- fresh_var;
+          return
+            (M $ Tuple [], as1 ⋓ as2 ⋓ as3,
+              (Unify d ty3 $ CVar fresh)::(Unify d ty2 $ PrimTy Integer)::
+                (Unify d ty1 $ Array $ CVar fresh)::(cs1++cs2++cs3))
+          od
+      | _ => fail)
+
+    else if s = "True" ∨ s = "False" then (
+      case es of
+      | [] => return (PrimTy Bool, empty, [])
+      | _ => fail)
+
+    else if s = "Subscript" then (
+      case es of
+      | [] => return (Exception, empty, [])
+      | _ => fail)
+
+    else do
+      (tys,as,cs) <- FOLDR
+            (λe acc. do
+                (tys, as, cs) <- acc;
+                (ty, as', cs') <- infer ns mset e;
+                return (ty::tys, as ⋓ as', cs' ++ cs) od)
+            (return ([],empty,[])) es;
+      case ALOOKUP (FST ns) s of
+      (* Exceptions *)
+      | SOME arg_tys => (
+          if LENGTH arg_tys = LENGTH tys then
+            return (Exception, as,
+                    (list$MAP2 (λt a. Unify d t $ itype_of a) tys arg_tys) ++ cs)
+          else fail)
+      | NONE => case infer_cons 0 (SND ns) s of
+      (* Constructors *)
+      | SOME (n, ar, arg_tys) => (
+          if LENGTH arg_tys = LENGTH tys then do
+            freshes <- fresh_vars ar;
+            cfreshes <<- MAP CVar freshes;
+            return (TypeCons n cfreshes, as,
+            (MAP (λcf. Unify d cf cf) cfreshes ++
+             list$MAP2
+              (λt a. Unify d t (isubst cfreshes $ itype_of a)) tys arg_tys) ++ cs) od
+          else fail)
+      | NONE => fail od) ∧
+
+  infer ns mset (Prim d (AtomOp aop) es) = do
+    (arg_tys, ret_ty) <- oreturn $ infer_atom_op (LENGTH es) aop;
+    (tys, as, cs) <- FOLDR
+          (λe acc. do
+              (tys, as, cs) <- acc;
+              (ty, as', cs') <- infer ns mset e;
+              return (ty::tys, as ⋓ as', cs' ++ cs) od)
+          (return ([],empty,[])) es;
+    return (PrimTy ret_ty, as,
+            (list$MAP2 (λt a. Unify d t (PrimTy a)) tys arg_tys) ++ cs) od ∧
+
+  infer ns mset (Prim d Seq [e1;e2]) = do
+    (ty2, as2, cs2) <- infer ns mset e2;
+    (ty1, as1, cs1) <- infer ns mset e1;
+    return (ty2, as1 ⋓ as2, cs1++cs2) od ∧
+
+  infer ns mset (App d e es) = (
+    if NULL es then fail else do
+    (tys, as, cs) <- FOLDR
+          (λe acc. do
+              (tys, as, cs) <- acc;
+              (ty, as', cs') <- infer ns mset e;
+              return (ty::tys, as ⋓ as', cs' ++ cs) od)
+          (return ([],empty,[])) es;
+    (tyf, asf, csf) <- infer ns mset e;
+    fresh <- fresh_var;
+    return (CVar fresh, as ⋓ asf,
+            (Unify d tyf (iFunctions tys $ CVar fresh))::(csf ++ cs)) od) ∧
+
+  infer ns mset (Lam d xs e) = (
+    if NULL xs then fail else do
+    freshes <- fresh_vars (LENGTH xs);
+    cfreshes <<- MAP CVar freshes;
+    (ty, as, cs) <- infer ns (list_insert freshes mset) e;
+    return (iFunctions cfreshes ty, list_delete as xs,
+            MAP (λcf. Unify d cf cf) cfreshes ++
+            FLAT (list$MAP2
+              (λf x. MAP (Unify d (CVar f) o CVar) $ get_assumptions x as)
+            freshes xs) ++ cs) od) ∧
+
+  infer ns mset (Let d x e1 e2) = do
+    (ty2, as2, cs2) <- infer ns mset e2;
+    (ty1, as1, cs1) <- infer ns mset e1;
+    return (ty2, as1 ⋓ (delete as2 x),
+            (MAP (λn. Implicit d (CVar n) mset ty1) $ get_assumptions x as2) ++
+              cs1 ++ cs2) od ∧
+
+  infer ns mset (Letrec d fns e) = (
+    if NULL fns then fail else do
+    (tye, ase, cse) <- infer ns mset e;
+    (tyfns, asfns, csfns) <- FOLDR
+          (λ(fn,e) acc. do
+              (tys, as, cs) <- acc;
+              (ty, as', cs') <- infer ns mset e;
+              return (ty::tys, as ⋓ as', cs' ++ cs) od)
+          (return ([],empty,[])) fns;
+    return (tye, list_delete (ase ⋓ asfns) (MAP FST fns),
+            MAP (λt. Unify d t t) tyfns ++
+            (FLAT $ list$MAP2
+                (λ(x,b) tyfn. MAP (λn. Implicit d (CVar n) mset tyfn) $
+                                              get_assumptions x (ase ⋓ asfns))
+                fns tyfns) ++
+            csfns ++ cse) od) ∧
+
+  (* TODO check handling of variables *)
+  infer ns mset (Case d e v css) = (
+    if MEM v (FLAT (MAP (FST o SND) css)) then fail else
+    case css of
+    | [] => fail (* no empty case statements *)
+    | [("", pvars, rest)] => do (* tuple pattern match *)
+      fresh_v <- fresh_var;
+      cfresh_v <<- CVar fresh_v;
+      fresh_tyargs <- fresh_vars (LENGTH pvars);
+      cfresh_tyargs <<- MAP CVar fresh_tyargs;
+      (tyrest, asrest, csrest) <-
+        infer ns (list_insert (fresh_v::fresh_tyargs) mset) rest;
+      (tye, ase, cse) <- infer ns mset e;
+      pvar_constraints <<- list$MAP2
+        (λv t. MAP (λn. Unify d (CVar n) t) $ get_assumptions v asrest)
+          (v::pvars) (cfresh_v::cfresh_tyargs);
+      return (tyrest, ase ⋓ (list_delete asrest (v :: pvars)),
+                (Unify d cfresh_v tye)::(Unify d tye (Tuple cfresh_tyargs))::
+                (FLAT pvar_constraints) ++ cse ++ csrest) od
+
+    | _::_ => do
+      (id, ar, cdefs) <- oreturn (get_typedef 0 (SND ns)
+                                    (MAP (λ(cn,pvs,_). (cn, LENGTH pvs)) css));
+      fresh_v <- fresh_var;
+      cfresh_v <<- CVar fresh_v;
+      fresh_tyargs <- fresh_vars ar;
+      cfresh_tyargs <<- MAP CVar fresh_tyargs;
+      mono_vars <<- fresh_v::fresh_tyargs;
+      expected_arg_tys <<-
+        MAP (λ(cn,ts). (cn, MAP (isubst cfresh_tyargs o itype_of) ts)) cdefs;
+      (tys, as, cs) <- FOLDR
+            (λ(cname,pvars,rest) acc. do
+                (tys, as, cs) <- acc;
+                (ty, as', cs') <- infer ns (list_insert mono_vars mset) rest;
+                expected_cname_arg_tys <- oreturn (ALOOKUP expected_arg_tys cname);
+                pvar_constraints <<- list$MAP2
+                  (λv t. MAP (λn. Unify d (CVar n) t) $ get_assumptions v as')
+                    (v::pvars) (cfresh_v::expected_cname_arg_tys);
+                return (ty::tys, ((list_delete as' (v :: pvars)) ⋓ as),
+                        (FLAT pvar_constraints) ++ cs' ++ cs) od)
+            (return ([],empty,[])) css;
+      (tye, ase, cse) <- infer ns mset e;
+
+      return (HD tys, ase ⋓ as,
+              (Unify d cfresh_v tye)::(Unify d tye (TypeCons id cfresh_tyargs))::
+              (MAP (λt. Unify d (HD tys) t) (TL tys)) ++ cse ++ cs) od) ∧
+
+  infer _ _ _ = fail
+Termination
+  WF_REL_TAC `measure ( λ(_,_,e). cexp_size (K 0) e)` >> rw[] >>
+  rename1 `MEM _ es` >> pop_assum mp_tac >> rpt $ pop_assum kall_tac >>
+  Induct_on `es` >> rw[] >> gvs[cexp_size_def]
+End
+
+
+(******************** Constraint solving ********************)
+
+(*
+  Generalise CVars greater than/equal to `cv`, starting at deBruijn index `db`.
+  Avoid generalising the CVars given by `avoid`.
+  Return the number generalised, the generalised type, and a substitution
+  encapsulating the generalisation.
+*)
+Definition generalise_def:
+  generalise db (avoid : num_set) s (DBVar n) = (0n, s, DBVar n) ∧
+  generalise db avoid s (PrimTy p) = (0, s, PrimTy p) ∧
+  generalise db avoid s  Exception = (0, s, Exception) ∧
+
+  generalise db avoid s (TypeCons id ts) = (
+    let (n, s', ts') = generalise_list db avoid s ts in (n, s', TypeCons id ts')) ∧
+
+  generalise db avoid s (Tuple ts) = (
+    let (n, s', ts') = generalise_list db avoid s ts in (n, s', Tuple ts')) ∧
+
+  generalise db avoid s (Function t1 t2) = (
+    let (n1, s', t1') = generalise db avoid s t1 in
+    let (n2, s'', t2') = generalise (db + n1) avoid s' t2 in
+    (n1 + n2, s'', Function t1' t2')) ∧
+
+  generalise db avoid s (Array t) = (
+    let (n, s', t') = generalise db avoid s t in (n, s', Array t')) ∧
+
+  generalise db avoid s (M t) = (
+    let (n, s', t') = generalise db avoid s t in (n, s', M t')) ∧
+
+  generalise db avoid s (CVar c) = (
+    if lookup c avoid = NONE then (
+      case FLOOKUP s c of
+      | SOME n => (0, s, DBVar n)
+      | NONE => (1, s |+ (c,db), DBVar db))
+    else (0, s, CVar c)) ∧
+
+  generalise_list db avoid s [] = (0, s, []) ∧
+  generalise_list db avoid s (t::ts) =
+    let (n, s', t') = generalise db avoid s t in
+    let (ns, s'', ts') = generalise_list (db + n) avoid s' ts in
+    (n + ns, s'', t'::ts')
+End
+
+Definition freecvars_def:
+  freecvars (DBVar n) = LN ∧
+  freecvars (PrimTy p) = LN ∧
+  freecvars  Exception = LN ∧
+  freecvars (TypeCons id ts) = FOLDL union LN (MAP freecvars ts) ∧
+  freecvars (Tuple ts) = FOLDL union LN (MAP freecvars ts) ∧
+  freecvars (Function t1 t2) = union (freecvars t1) (freecvars t2) ∧
+  freecvars (Array t) = freecvars t ∧
+  freecvars (M t) = freecvars t ∧
+  freecvars (CVar n) = insert n () LN
+Termination
+  WF_REL_TAC `measure itype_size` >> rw[itype_size_def] >>
+  rename1 `MEM _ ts` >> Induct_on `ts` >> rw[itype_size_def] >> gvs[]
+End
+
+Definition subst_vars_def:
+  subst_vars s (vars : num_set) =
+    foldi (λn u acc. union acc $ freecvars $ pure_walkstar s (CVar n)) 0 LN vars
+End
+
+Definition subst_constraint_def:
+  subst_constraint s (Unify d t1 t2) =
+    Unify d (pure_walkstar s t1) (pure_walkstar s t2) ∧
+  subst_constraint s (Instantiate d t1 (vars, t2)) =
+    Instantiate d (pure_walkstar s t1) (vars, pure_walkstar s t2) ∧
+  subst_constraint s (Implicit d t1 vs t2) =
+    Implicit d (pure_walkstar s t1) (subst_vars s vs) (pure_walkstar s t2)
+End
+
+Definition activevars_def:
+  activevars (Unify d t1 t2) = union (freecvars t1) (freecvars t2) ∧
+  activevars (Implicit d t1 vars t2) =
+    union (freecvars t1) (inter vars (freecvars t2)) ∧
+  activevars (Instantiate d t (vars, scheme)) =
+    union (freecvars t) (freecvars scheme)
+End
+
+
+(* TODO this approach is naive *)
+
+Definition is_solveable_def:
+  is_solveable (Unify d t1 t2) cs = T ∧
+  is_solveable (Instantiate d t sch) cs = T ∧
+  is_solveable (Implicit d t1 vars t2) cs =
+    let active = FOLDL (λacc c. union (activevars c) acc) LN
+                  (Implicit d t1 vars t2 :: cs) in
+    difference (inter (freecvars t2) active) vars = LN
+End
+
+(* TODO reverse shouldn't be necessary here *)
+Definition get_solveable_def:
+  get_solveable [] cs = NONE ∧
+  get_solveable (c::rest) cs =
+    if is_solveable c (REVERSE cs ++ rest) then
+      SOME (c, REVERSE cs ++ rest)
+    else get_solveable rest (c::cs)
+End
+
+Theorem get_solveable_SOME:
+  ∀cs rev_cs c cs'.
+    get_solveable cs rev_cs = SOME (c, cs')
+  ⇒ ∃left right.
+      cs = left ++ [c] ++ right ∧
+      cs' = REVERSE rev_cs ++ left ++ right ∧
+      is_solveable c cs'
+Proof
+  Induct >> rw[get_solveable_def] >> simp[]
+  >- (qexists_tac `[]` >> simp[]) >>
+  last_x_assum drule >> rw[] >> qexists_tac `h::left` >> simp[]
+QED
+
+Definition constraint_weight_def:
+  constraint_weight (Unify _ _ _) = 1n ∧
+  constraint_weight (Instantiate _ _ _ ) = 2n ∧
+  constraint_weight (Implicit _ _ _ _ ) = 3n
+End
+
+Theorem constraint_weight_subst_constraint[simp]:
+  ∀t s. constraint_weight (subst_constraint s t) = constraint_weight t
+Proof
+  Cases >> rw[subst_constraint_def, constraint_weight_def] >>
+  PairCases_on `p` >> rw[subst_constraint_def, constraint_weight_def]
+QED
+
+Definition solve_def:
+  solve [] = return FEMPTY ∧
+
+  solve cs = case get_solveable cs [] of
+    | NONE => fail
+
+    | SOME $ (Unify d t1 t2, cs) => do
+        sub <- oreturn $ pure_unify FEMPTY t1 t2;
+        cs' <<- MAP (subst_constraint sub) cs;
+        solve_rest <- solve cs';
+        return (FUNION sub solve_rest) od
+
+    | SOME $ (Instantiate d t (vs, scheme), cs) => do
+        freshes <- fresh_vars vs;
+        inst_scheme <<- isubst (MAP CVar freshes) scheme;
+        solve (Unify d t inst_scheme :: cs) od
+
+    | SOME $ (Implicit d t1 vs t2, cs) => do
+        (n, s, scheme) <<- generalise 0 vs FEMPTY t2;
+        solve (Instantiate d t1 (n, scheme) :: cs) od
+Termination
+  WF_REL_TAC `measure $ λl. SUM $ MAP constraint_weight l` >>
+  rw[constraint_weight_def, MAP_MAP_o, combinTheory.o_DEF, SF ETA_ss] >>
+  drule get_solveable_SOME >> strip_tac >> gvs[] >>
+  Cases_on `left` >> gvs[SUM_APPEND, constraint_weight_def]
+End
+
+Definition infer_top_level_def:
+  infer_top_level ns d cexp = do
+    (ty, as, cs) <- infer ns LN cexp;
+    if ¬ null as then fail else return ();
+    solve (Unify d ty (M Unit) :: cs)
+  od 0
+End
+
+
+(********************)
+
+val _ = export_theory();
