typing/pure_inference_commonScript.sml
@@ -1,0 +1,160 @@
+(* Definitions common to inference theories. *)
+open HolKernel Parse boolLib bossLib BasicProvers dep_rewrite;
+open arithmeticTheory optionTheory listTheory;
+open pure_typingTheory;
+
+val _ = new_theory "pure_inference_common";
+
+Datatype:
+  itype = DBVar num
+        | PrimTy prim_ty
+        | Exception
+        | TypeCons num (itype list)
+        | Tuple (itype list)
+        | Function itype itype
+        | Array itype
+        | M itype
+        | CVar num
+End
+
+Overload Unit = ``Tuple []``;
+Overload IntTy = ``PrimTy Integer``;
+Overload BoolTy = ``PrimTy Bool``;
+Overload StrTy = ``PrimTy String``;
+
+Theorem itype_ind:
+  ∀P.
+    (∀n. P (DBVar n)) ∧ (∀p. P (PrimTy p)) ∧ P Exception ∧
+    (∀id ts. (∀a. MEM a ts ⇒ P a) ⇒ P (TypeCons id ts)) ∧
+    (∀ts. (∀a. MEM a ts ⇒ P a) ⇒ P (Tuple ts)) ∧
+    (∀t1 t2. P t1 ∧ P t2 ⇒ P (Function t1 t2)) ∧
+    (∀t. P t ⇒ P (Array t)) ∧ (∀t. P t ⇒ P (M t)) ∧ (∀n. P (CVar n))
+  ⇒ ∀v. P v
+Proof
+  ntac 3 strip_tac >>
+  completeInduct_on `itype_size v` >> rw[] >>
+  Cases_on `v` >> gvs[fetch "-" "itype_size_def"] >>
+  last_x_assum irule >> rw[] >>
+  first_x_assum irule >> simp[] >>
+  Induct_on `l` >> rw[] >> gvs[fetch "-" "itype_size_def"]
+QED
+
+Definition iFunctions_def:
+  iFunctions [] t = t ∧
+  iFunctions (at::ats) t = Function at (iFunctions ats t)
+End
+
+Definition freedbvars_def:
+  (freedbvars (DBVar n) = {n}) ∧
+  (freedbvars (PrimTy pty) = {}) ∧
+  (freedbvars Exception = {}) ∧
+  (freedbvars (TypeCons id its) = BIGUNION (set (MAP freedbvars its))) ∧
+  (freedbvars (Tuple its) = BIGUNION (set (MAP freedbvars its))) ∧
+  (freedbvars (Function it1 it2) = freedbvars it1 ∪ freedbvars it2) ∧
+  (freedbvars (Array it) = freedbvars it) ∧
+  (freedbvars (M it) = freedbvars it) ∧
+  (freedbvars (CVar cv) = {})
+Termination
+  WF_REL_TAC `measure itype_size` >> rw[fetch "-" "itype_size_def"] >>
+  rename1 `MEM a its` >> Induct_on `its` >> rw[] >> gvs[fetch "-" "itype_size_def"]
+End
+
+Definition itype_wf_def:
+  itype_wf (typedefs : typedefs) (DBVar n) = T ∧
+  itype_wf typedefs (PrimTy pty) = T ∧
+  itype_wf typedefs  Exception = T ∧
+  itype_wf typedefs (TypeCons id tyargs) = (
+    EVERY (itype_wf typedefs) tyargs ∧
+    ∃arity constructors.
+      (* Type definition exists: *)
+        oEL id typedefs = SOME (arity, constructors) ∧
+      (* And has correct arity: *)
+        LENGTH tyargs = arity) ∧
+  itype_wf typedefs (Tuple ts) =
+    EVERY (itype_wf typedefs) ts ∧
+  itype_wf typedefs (Function tf t) = (
+    itype_wf typedefs t ∧ itype_wf typedefs tf) ∧
+  itype_wf typedefs (Array t) = itype_wf typedefs t ∧
+  itype_wf typedefs (M t) = itype_wf typedefs t ∧
+  itype_wf typedefs (CVar cv) = T
+Termination
+  WF_REL_TAC `measure (itype_size o SND)` >> rw[fetch "-" "itype_size_def"] >>
+  rename1 `MEM _ ts` >> Induct_on `ts` >> rw[fetch "-" "itype_size_def"] >> gvs[]
+End
+
+Definition itype_ok_def:
+  itype_ok typedefs db t ⇔
+    freedbvars t ⊆ count db ∧
+    itype_wf typedefs t
+End
+
+Definition isubst_def:
+  isubst ts (DBVar v) = (
+    if v < LENGTH ts then EL v ts else DBVar (v - LENGTH ts)) ∧
+  isubst ts (PrimTy p) = PrimTy p ∧
+  isubst ts  Exception = Exception ∧
+  isubst ts (TypeCons n tcs) = TypeCons n (MAP (isubst ts) tcs) ∧
+  isubst ts (Tuple tcs) = Tuple  (MAP (isubst ts) tcs) ∧
+  isubst ts (Function tf t) =
+    Function (isubst ts tf) (isubst ts t) ∧
+  isubst ts (Array t) = Array (isubst ts t) ∧
+  isubst ts (M t) = M (isubst ts t) ∧
+  isubst ts (CVar c) = CVar c
+Termination
+  WF_REL_TAC `measure (itype_size o SND)` >> rw[fetch "-" "itype_size_def"] >>
+  rename1 `MEM _ ts` >> Induct_on `ts` >> rw[fetch "-" "itype_size_def"] >> gvs[]
+End
+
+Definition ishift_def:
+  ishift n (DBVar v) = DBVar (v + n) ∧
+  ishift n (PrimTy p) = PrimTy p ∧
+  ishift n  Exception = Exception ∧
+  ishift n (TypeCons tn tcs) = TypeCons tn (MAP (ishift n) tcs) ∧
+  ishift n (Tuple tcs) = Tuple  (MAP (ishift n) tcs) ∧
+  ishift n (Function tf t) =
+    Function (ishift n tf) (ishift n t) ∧
+  ishift n (Array t) = Array (ishift n t) ∧
+  ishift n (M t) = M (ishift n t) ∧
+  ishift n (CVar c) = CVar c
+Termination
+  WF_REL_TAC `measure (itype_size o SND)` >> rw[fetch "-" "itype_size_def"] >>
+  rename1 `MEM _ ts` >> Induct_on `ts` >> rw[fetch "-" "itype_size_def"] >> gvs[]
+End
+
+Definition itype_of_def:
+  itype_of (TypeVar n) = DBVar n ∧
+  itype_of (PrimTy p) = PrimTy p ∧
+  itype_of Exception = Exception ∧
+  itype_of (TypeCons n ts) = TypeCons n (MAP itype_of ts) ∧
+  itype_of (Tuple ts) = Tuple (MAP itype_of ts) ∧
+  itype_of (Function t1 t2) = Function (itype_of t1) (itype_of t2) ∧
+  itype_of (Array t) = Array (itype_of t) ∧
+  itype_of (M t) = M (itype_of t)
+Termination
+  WF_REL_TAC `measure type_size` >> rw[type_size_def] >>
+  rename1 `MEM _ ts` >> Induct_on `ts` >> rw[] >> gvs[type_size_def]
+End
+
+Definition type_of_def:
+  type_of (DBVar n) = SOME $ TypeVar n ∧
+  type_of (PrimTy p) = SOME $ PrimTy p ∧
+  type_of Exception = SOME $ Exception ∧
+  type_of (TypeCons n ts) =
+    OPTION_MAP (TypeCons n) $
+      FOLDR (λt ts_opt. OPTION_MAP2 CONS (type_of t) ts_opt) (SOME []) ts ∧
+  type_of (Tuple ts) =
+    OPTION_MAP Tuple $
+      FOLDR (λt ts_opt. OPTION_MAP2 CONS (type_of t) ts_opt) (SOME []) ts ∧
+  type_of (Function t1 t2) =
+    OPTION_BIND (type_of t1)
+    (λit1. OPTION_BIND (type_of t2) (λit2. SOME $ Function it1 it2)) ∧
+  type_of (Array t) = OPTION_MAP Array (type_of t) ∧
+  type_of (M t) = OPTION_MAP M (type_of t) ∧
+  type_of (CVar n) = NONE
+Termination
+  WF_REL_TAC `measure itype_size` >> rw[fetch "-" "itype_size_def"] >>
+  rename1 `MEM _ ts` >> Induct_on `ts` >> rw[fetch "-" "itype_size_def"] >> gvs[]
+End
+
+val _ = export_theory();
+
